src/HOL/TLA/Memory/MemoryImplementation.thy
@@ -3,12 +3,9 @@
     ID:          $Id$
     Author:      Stephan Merz
     Copyright:   1997 University of Munich
-
-    Theory Name: MemoryImplementation
-    Logic Image: TLA
-
-    RPC-Memory example: Memory implementation
 *)
+
+header {* RPC-Memory example: Memory implementation *}
 
 theory MemoryImplementation
 imports Memory RPC MemClerk
@@ -177,6 +174,1143 @@ axioms
                            (rtrner crCh!p, caller rmCh!p, rst!p),
                            (mm!l, rtrner rmCh!p, ires!p))"
 
-ML {* use_legacy_bindings (the_context ()) *}
+(*
+    The main theorem is theorem "Implementation" at the end of this file,
+    which shows that the composition of a reliable memory, an RPC component, and
+    a memory clerk implements an unreliable memory. The files "MIsafe.ML" and
+    "MIlive.ML" contain lower-level lemmas for the safety and liveness parts.
+
+    Steps are (roughly) numbered as in the hand proof.
+*)
+
+(* --------------------------- automatic prover --------------------------- *)
+
+declare if_weak_cong [cong del]
+
+ML {* val MI_css = (claset(), simpset()) *}
+
+(* A more aggressive variant that tries to solve subgoals by assumption
+   or contradiction during the simplification.
+   THIS IS UNSAFE, BECAUSE IT DOESN'T RECORD THE CHOICES!!
+   (but it can be a lot faster than MI_css)
+*)
+
+ML {*
+val MI_fast_css =
+  let
+    val (cs,ss) = MI_css
+  in
+    (cs addSEs [temp_use (thm "squareE")],
+      ss addSSolver (mk_solver "" (fn thms => assume_tac ORELSE' (etac notE))))
+  end;
+
+val temp_elim = make_elim o temp_use;
+*}
+
+
+
+(****************************** The history variable ******************************)
+
+section "History variable"
+
+lemma HistoryLemma: "|- Init(ALL p. ImpInit p) & [](ALL p. ImpNext p)
+         --> (EEX rmhist. Init(ALL p. HInit rmhist p)
+                          & [](ALL p. [HNext rmhist p]_(c p, r p, m p, rmhist!p)))"
+  apply clarsimp
+  apply (rule historyI)
+      apply assumption+
+  apply (rule MI_base)
+  apply (tactic {* action_simp_tac (simpset () addsimps [thm "HInit_def"]) [] [] 1 *})
+   apply (erule fun_cong)
+  apply (tactic {* action_simp_tac (simpset () addsimps [thm "HNext_def"])
+    [thm "busy_squareI"] [] 1 *})
+  apply (erule fun_cong)
+  done
+
+lemma History: "|- Implementation --> (EEX rmhist. Hist rmhist)"
+  apply clarsimp
+  apply (rule HistoryLemma [temp_use, THEN eex_mono])
+    prefer 3
+    apply (force simp: Hist_def HistP_def Init_def all_box [try_rewrite]
+      split_box_conj [try_rewrite])
+   apply (auto simp: Implementation_def MClkISpec_def RPCISpec_def
+     IRSpec_def MClkIPSpec_def RPCIPSpec_def RPSpec_def ImpInit_def
+     Init_def ImpNext_def c_def r_def m_def all_box [temp_use] split_box_conj [temp_use])
+  done
+
+(******************************** The safety part *********************************)
+
+section "The safety part"
+
+(* ------------------------- Include lower-level lemmas ------------------------- *)
+
+(* RPCFailure notin MemVals U {OK,BadArg} *)
+
+lemma MVOKBAnotRF: "MVOKBA x ==> x ~= RPCFailure"
+  apply (unfold MVOKBA_def)
+  apply auto
+  done
+
+(* NotAResult notin MemVals U {OK,BadArg,RPCFailure} *)
+
+lemma MVOKBARFnotNR: "MVOKBARF x ==> x ~= NotAResult"
+  apply (unfold MVOKBARF_def)
+  apply auto
+  done
+
+(* ================ Si's are mutually exclusive ================================ *)
+(* Si and Sj are mutually exclusive for i # j. This helps to simplify the big
+   conditional in the definition of resbar when doing the step-simulation proof.
+   We prove a weaker result, which suffices for our purposes:
+   Si implies (not Sj), for j<i.
+*)
+
+(* --- not used ---
+Goal "|- S1 rmhist p --> S1 rmhist p & ~S2 rmhist p & ~S3 rmhist p &
+                         ~S4 rmhist p & ~S5 rmhist p & ~S6 rmhist p"
+by (auto_tac (MI_css addsimps2 [S_def, S1_def, S2_def,
+                                S3_def, S4_def, S5_def, S6_def]));
+qed "S1_excl";
+*)
+
+lemma S2_excl: "|- S2 rmhist p --> S2 rmhist p & ~S1 rmhist p"
+  by (auto simp: S_def S1_def S2_def)
+
+lemma S3_excl: "|- S3 rmhist p --> S3 rmhist p & ~S1 rmhist p & ~S2 rmhist p"
+  by (auto simp: S_def S1_def S2_def S3_def)
+
+lemma S4_excl: "|- S4 rmhist p --> S4 rmhist p & ~S1 rmhist p & ~S2 rmhist p & ~S3 rmhist p"
+  by (auto simp: S_def S1_def S2_def S3_def S4_def)
+
+lemma S5_excl: "|- S5 rmhist p --> S5 rmhist p & ~S1 rmhist p & ~S2 rmhist p
+                         & ~S3 rmhist p & ~S4 rmhist p"
+  by (auto simp: S_def S1_def S2_def S3_def S4_def S5_def)
+
+lemma S6_excl: "|- S6 rmhist p --> S6 rmhist p & ~S1 rmhist p & ~S2 rmhist p
+                         & ~S3 rmhist p & ~S4 rmhist p & ~S5 rmhist p"
+  by (auto simp: S_def S1_def S2_def S3_def S4_def S5_def S6_def)
+
+
+(* ==================== Lemmas about the environment ============================== *)
+
+lemma Envbusy: "|- $(Calling memCh p) --> ~ENext p"
+  by (auto simp: ENext_def Call_def)
+
+(* ==================== Lemmas about the implementation's states ==================== *)
+
+(* The following series of lemmas are used in establishing the implementation's
+   next-state relation (Step 1.2 of the proof in the paper). For each state Si, we
+   determine which component actions are possible and what state they result in.
+*)
+
+(* ------------------------------ State S1 ---------------------------------------- *)
+
+lemma S1Env: "|- ENext p & $(S1 rmhist p) & unchanged (c p, r p, m p, rmhist!p)
+         --> (S2 rmhist p)$"
+  by (force simp: ENext_def Call_def c_def r_def m_def
+    caller_def rtrner_def MVNROKBA_def S_def S1_def S2_def Calling_def)
+
+lemma S1ClerkUnch: "|- [MClkNext memCh crCh cst p]_(c p) & $(S1 rmhist p) --> unchanged (c p)"
+  by (tactic {* auto_tac (MI_fast_css addSDs2 [temp_use (thm "MClkidle")]
+    addsimps2 [thm "S_def", thm "S1_def"]) *})
+
+lemma S1RPCUnch: "|- [RPCNext crCh rmCh rst p]_(r p) & $(S1 rmhist p) --> unchanged (r p)"
+  by (tactic {* auto_tac (MI_fast_css addSDs2 [temp_use (thm "RPCidle")]
+    addsimps2 [thm "S_def", thm "S1_def"]) *})
+
+lemma S1MemUnch: "|- [RNext rmCh mm ires p]_(m p) & $(S1 rmhist p) --> unchanged (m p)"
+  by (tactic {* auto_tac (MI_fast_css addSDs2 [temp_use (thm "Memoryidle")]
+    addsimps2 [thm "S_def", thm "S1_def"]) *})
+
+lemma S1Hist: "|- [HNext rmhist p]_(c p,r p,m p,rmhist!p) & $(S1 rmhist p)
+         --> unchanged (rmhist!p)"
+  by (tactic {* action_simp_tac (simpset () addsimps [thm "HNext_def", thm "S_def",
+    thm "S1_def", thm "MemReturn_def", thm "RPCFail_def", thm "MClkReply_def",
+    thm "Return_def"]) [] [temp_use (thm "squareE")] 1 *})
+
+
+(* ------------------------------ State S2 ---------------------------------------- *)
+
+lemma S2EnvUnch: "|- [ENext p]_(e p) & $(S2 rmhist p) --> unchanged (e p)"
+  by (auto dest!: Envbusy [temp_use] simp: S_def S2_def)
+
+lemma S2Clerk: "|- MClkNext memCh crCh cst p & $(S2 rmhist p) --> MClkFwd memCh crCh cst p"
+  by (auto simp: MClkNext_def MClkRetry_def MClkReply_def S_def S2_def)
+
+lemma S2Forward: "|- $(S2 rmhist p) & MClkFwd memCh crCh cst p
+         & unchanged (e p, r p, m p, rmhist!p)
+         --> (S3 rmhist p)$"
+  by (tactic {* action_simp_tac (simpset () addsimps [thm "MClkFwd_def",
+    thm "Call_def", thm "e_def", thm "r_def", thm "m_def", thm "caller_def",
+    thm "rtrner_def", thm "S_def", thm "S2_def", thm "S3_def", thm "Calling_def"]) [] [] 1 *})
+
+lemma S2RPCUnch: "|- [RPCNext crCh rmCh rst p]_(r p) & $(S2 rmhist p) --> unchanged (r p)"
+  by (auto simp: S_def S2_def dest!: RPCidle [temp_use])
+
+lemma S2MemUnch: "|- [RNext rmCh mm ires p]_(m p) & $(S2 rmhist p) --> unchanged (m p)"
+  by (auto simp: S_def S2_def dest!: Memoryidle [temp_use])
+
+lemma S2Hist: "|- [HNext rmhist p]_(c p,r p,m p,rmhist!p) & $(S2 rmhist p)
+         --> unchanged (rmhist!p)"
+  by (tactic {* auto_tac (MI_fast_css addsimps2 [thm "HNext_def", thm "MemReturn_def",
+    thm "RPCFail_def", thm "MClkReply_def", thm "Return_def", thm "S_def", thm "S2_def"]) *})
+
+(* ------------------------------ State S3 ---------------------------------------- *)
+
+lemma S3EnvUnch: "|- [ENext p]_(e p) & $(S3 rmhist p) --> unchanged (e p)"
+  by (auto dest!: Envbusy [temp_use] simp: S_def S3_def)
+
+lemma S3ClerkUnch: "|- [MClkNext memCh crCh cst p]_(c p) & $(S3 rmhist p) --> unchanged (c p)"
+  by (auto dest!: MClkbusy [temp_use] simp: square_def S_def S3_def)
+
+lemma S3LegalRcvArg: "|- S3 rmhist p --> IsLegalRcvArg<arg<crCh!p>>"
+  by (auto simp: IsLegalRcvArg_def MClkRelayArg_def S_def S3_def)
+
+lemma S3RPC: "|- RPCNext crCh rmCh rst p & $(S3 rmhist p)
+         --> RPCFwd crCh rmCh rst p | RPCFail crCh rmCh rst p"
+  apply clarsimp
+  apply (frule S3LegalRcvArg [action_use])
+  apply (auto simp: RPCNext_def RPCReject_def RPCReply_def S_def S3_def)
+  done
+
+lemma S3Forward: "|- RPCFwd crCh rmCh rst p & HNext rmhist p & $(S3 rmhist p)
+         & unchanged (e p, c p, m p)
+         --> (S4 rmhist p)$ & unchanged (rmhist!p)"
+  by (tactic {* action_simp_tac (simpset () addsimps [thm "RPCFwd_def",
+    thm "HNext_def", thm "MemReturn_def", thm "RPCFail_def",
+    thm "MClkReply_def", thm "Return_def", thm "Call_def", thm "e_def",
+    thm "c_def", thm "m_def", thm "caller_def", thm "rtrner_def", thm "S_def",
+    thm "S3_def", thm "S4_def", thm "Calling_def"]) [] [] 1 *})
+
+lemma S3Fail: "|- RPCFail crCh rmCh rst p & $(S3 rmhist p) & HNext rmhist p
+         & unchanged (e p, c p, m p)
+         --> (S6 rmhist p)$"
+  by (tactic {* action_simp_tac (simpset () addsimps [thm "HNext_def",
+    thm "RPCFail_def", thm "Return_def", thm "e_def", thm "c_def",
+    thm "m_def", thm "caller_def", thm "rtrner_def", thm "MVOKBARF_def",
+    thm "S_def", thm "S3_def", thm "S6_def", thm "Calling_def"]) [] [] 1 *})
+
+lemma S3MemUnch: "|- [RNext rmCh mm ires p]_(m p) & $(S3 rmhist p) --> unchanged (m p)"
+  by (auto simp: S_def S3_def dest!: Memoryidle [temp_use])
+
+lemma S3Hist: "|- HNext rmhist p & $(S3 rmhist p) & unchanged (r p) --> unchanged (rmhist!p)"
+  by (auto simp: HNext_def MemReturn_def RPCFail_def MClkReply_def
+    Return_def r_def rtrner_def S_def S3_def Calling_def)
+
+(* ------------------------------ State S4 ---------------------------------------- *)
+
+lemma S4EnvUnch: "|- [ENext p]_(e p) & $(S4 rmhist p) --> unchanged (e p)"
+  by (auto simp: S_def S4_def dest!: Envbusy [temp_use])
+
+lemma S4ClerkUnch: "|- [MClkNext memCh crCh cst p]_(c p) & $(S4 rmhist p) --> unchanged (c p)"
+  by (auto simp: S_def S4_def dest!: MClkbusy [temp_use])
+
+lemma S4RPCUnch: "|- [RPCNext crCh rmCh rst p]_(r p) & $(S4 rmhist p) --> unchanged (r p)"
+  by (tactic {* auto_tac (MI_fast_css addsimps2 [thm "S_def", thm "S4_def"]
+    addSDs2 [temp_use (thm "RPCbusy")]) *})
+
+lemma S4ReadInner: "|- ReadInner rmCh mm ires p l & $(S4 rmhist p) & unchanged (e p, c p, r p)
+         & HNext rmhist p & $(MemInv mm l)
+         --> (S4 rmhist p)$ & unchanged (rmhist!p)"
+  by (tactic {* action_simp_tac (simpset () addsimps [thm "ReadInner_def",
+    thm "GoodRead_def", thm "BadRead_def", thm "HNext_def", thm "MemReturn_def",
+    thm "RPCFail_def", thm "MClkReply_def", thm "Return_def", thm "e_def",
+    thm "c_def", thm "r_def", thm "rtrner_def", thm "caller_def",
+    thm "MVNROKBA_def", thm "S_def", thm "S4_def", thm "RdRequest_def",
+    thm "Calling_def", thm "MemInv_def"]) [] [] 1 *})
+
+lemma S4Read: "|- Read rmCh mm ires p & $(S4 rmhist p) & unchanged (e p, c p, r p)
+         & HNext rmhist p & (!l. $MemInv mm l)
+         --> (S4 rmhist p)$ & unchanged (rmhist!p)"
+  by (auto simp: Read_def dest!: S4ReadInner [temp_use])
+
+lemma S4WriteInner: "|- WriteInner rmCh mm ires p l v & $(S4 rmhist p) & unchanged (e p, c p, r p)           & HNext rmhist p
+         --> (S4 rmhist p)$ & unchanged (rmhist!p)"
+  by (tactic {* action_simp_tac (simpset () addsimps [thm "WriteInner_def",
+    thm "GoodWrite_def", thm "BadWrite_def", thm "HNext_def", thm "MemReturn_def",
+    thm "RPCFail_def", thm "MClkReply_def", thm "Return_def", thm "e_def",
+    thm "c_def", thm "r_def", thm "rtrner_def", thm "caller_def", thm "MVNROKBA_def",
+    thm "S_def", thm "S4_def", thm "WrRequest_def", thm "Calling_def"]) [] [] 1 *})
+
+lemma S4Write: "|- Write rmCh mm ires p l & $(S4 rmhist p) & unchanged (e p, c p, r p)
+         & (HNext rmhist p)
+         --> (S4 rmhist p)$ & unchanged (rmhist!p)"
+  by (auto simp: Write_def dest!: S4WriteInner [temp_use])
+
+lemma WriteS4: "|- $ImpInv rmhist p & Write rmCh mm ires p l --> $S4 rmhist p"
+  by (auto simp: Write_def WriteInner_def ImpInv_def
+    WrRequest_def S_def S1_def S2_def S3_def S4_def S5_def S6_def)
+
+lemma S4Return: "|- MemReturn rmCh ires p & $S4 rmhist p & unchanged (e p, c p, r p)
+         & HNext rmhist p
+         --> (S5 rmhist p)$"
+  by (auto simp: HNext_def MemReturn_def Return_def e_def c_def r_def
+    rtrner_def caller_def MVNROKBA_def MVOKBA_def S_def S4_def S5_def Calling_def)
+
+lemma S4Hist: "|- HNext rmhist p & $S4 rmhist p & (m p)$ = $(m p) --> (rmhist!p)$ = $(rmhist!p)"
+  by (auto simp: HNext_def MemReturn_def RPCFail_def MClkReply_def
+    Return_def m_def rtrner_def S_def S4_def Calling_def)
+
+(* ------------------------------ State S5 ---------------------------------------- *)
+
+lemma S5EnvUnch: "|- [ENext p]_(e p) & $(S5 rmhist p) --> unchanged (e p)"
+  by (auto simp: S_def S5_def dest!: Envbusy [temp_use])
+
+lemma S5ClerkUnch: "|- [MClkNext memCh crCh cst p]_(c p) & $(S5 rmhist p) --> unchanged (c p)"
+  by (auto simp: S_def S5_def dest!: MClkbusy [temp_use])
+
+lemma S5RPC: "|- RPCNext crCh rmCh rst p & $(S5 rmhist p)
+         --> RPCReply crCh rmCh rst p | RPCFail crCh rmCh rst p"
+  by (auto simp: RPCNext_def RPCReject_def RPCFwd_def S_def S5_def)
+
+lemma S5Reply: "|- RPCReply crCh rmCh rst p & $(S5 rmhist p) & unchanged (e p, c p, m p,rmhist!p)
+       --> (S6 rmhist p)$"
+  by (tactic {* action_simp_tac (simpset () addsimps [thm "RPCReply_def",
+    thm "Return_def", thm "e_def", thm "c_def", thm "m_def", thm "MVOKBA_def",
+    thm "MVOKBARF_def", thm "caller_def", thm "rtrner_def", thm "S_def",
+    thm "S5_def", thm "S6_def", thm "Calling_def"]) [] [] 1 *})
+
+lemma S5Fail: "|- RPCFail crCh rmCh rst p & $(S5 rmhist p) & unchanged (e p, c p, m p,rmhist!p)
+         --> (S6 rmhist p)$"
+  by (tactic {* action_simp_tac (simpset () addsimps [thm "RPCFail_def",
+    thm "Return_def", thm "e_def", thm "c_def", thm "m_def",
+    thm "MVOKBARF_def", thm "caller_def", thm "rtrner_def",
+    thm "S_def", thm "S5_def", thm "S6_def", thm "Calling_def"]) [] [] 1 *})
+
+lemma S5MemUnch: "|- [RNext rmCh mm ires p]_(m p) & $(S5 rmhist p) --> unchanged (m p)"
+  by (auto simp: S_def S5_def dest!: Memoryidle [temp_use])
+
+lemma S5Hist: "|- [HNext rmhist p]_(c p, r p, m p, rmhist!p) & $(S5 rmhist p)
+         --> (rmhist!p)$ = $(rmhist!p)"
+  by (tactic {* auto_tac (MI_fast_css addsimps2 [thm "HNext_def",
+    thm "MemReturn_def", thm "RPCFail_def", thm "MClkReply_def", thm "Return_def",
+    thm "S_def", thm "S5_def"]) *})
+
+(* ------------------------------ State S6 ---------------------------------------- *)
+
+lemma S6EnvUnch: "|- [ENext p]_(e p) & $(S6 rmhist p) --> unchanged (e p)"
+  by (auto simp: S_def S6_def dest!: Envbusy [temp_use])
+
+lemma S6Clerk: "|- MClkNext memCh crCh cst p & $(S6 rmhist p)
+         --> MClkRetry memCh crCh cst p | MClkReply memCh crCh cst p"
+  by (auto simp: MClkNext_def MClkFwd_def S_def S6_def)
+
+lemma S6Retry: "|- MClkRetry memCh crCh cst p & HNext rmhist p & $S6 rmhist p
+         & unchanged (e p,r p,m p)
+         --> (S3 rmhist p)$ & unchanged (rmhist!p)"
+  by (tactic {* action_simp_tac (simpset () addsimps [thm "HNext_def",
+    thm "MClkReply_def", thm "MClkRetry_def", thm "Call_def", thm "Return_def",
+    thm "e_def", thm "r_def", thm "m_def", thm "caller_def", thm "rtrner_def",
+    thm "S_def", thm "S6_def", thm "S3_def", thm "Calling_def"]) [] [] 1 *})
+
+lemma S6Reply: "|- MClkReply memCh crCh cst p & HNext rmhist p & $S6 rmhist p
+         & unchanged (e p,r p,m p)
+         --> (S1 rmhist p)$"
+  by (tactic {* action_simp_tac (simpset () addsimps [thm "HNext_def",
+    thm "MemReturn_def", thm "RPCFail_def", thm "Return_def", thm "MClkReply_def",
+    thm "e_def", thm "r_def", thm "m_def", thm "caller_def", thm "rtrner_def",
+    thm "S_def", thm "S6_def", thm "S1_def", thm "Calling_def"]) [] [] 1 *})
+
+lemma S6RPCUnch: "|- [RPCNext crCh rmCh rst p]_(r p) & $S6 rmhist p --> unchanged (r p)"
+  by (auto simp: S_def S6_def dest!: RPCidle [temp_use])
+
+lemma S6MemUnch: "|- [RNext rmCh mm ires p]_(m p) & $(S6 rmhist p) --> unchanged (m p)"
+  by (auto simp: S_def S6_def dest!: Memoryidle [temp_use])
+
+lemma S6Hist: "|- HNext rmhist p & $S6 rmhist p & (c p)$ = $(c p) --> (rmhist!p)$ = $(rmhist!p)"
+  by (auto simp: HNext_def MClkReply_def Return_def c_def rtrner_def S_def S6_def Calling_def)
+
+
+section "Correctness of predicate-action diagram"
+
+
+(* ========== Step 1.1 ================================================= *)
+(* The implementation's initial condition implies the state predicate S1 *)
+
+lemma Step1_1: "|- ImpInit p & HInit rmhist p --> S1 rmhist p"
+  by (tactic {* auto_tac (MI_fast_css addsimps2 [thm "MVNROKBA_def",
+    thm "MClkInit_def", thm "RPCInit_def", thm "PInit_def", thm "HInit_def",
+    thm "ImpInit_def", thm "S_def", thm "S1_def"]) *})
+
+(* ========== Step 1.2 ================================================== *)
+(* Figure 16 is a predicate-action diagram for the implementation. *)
+
+lemma Step1_2_1: "|- [HNext rmhist p]_(c p,r p,m p, rmhist!p) & ImpNext p
+         & ~unchanged (e p, c p, r p, m p, rmhist!p)  & $S1 rmhist p
+         --> (S2 rmhist p)$ & ENext p & unchanged (c p, r p, m p)"
+  apply (tactic {* action_simp_tac (simpset() addsimps [thm "ImpNext_def"]) []
+      (map temp_elim [thm "S1ClerkUnch", thm "S1RPCUnch", thm "S1MemUnch", thm "S1Hist"]) 1 *})
+   apply (tactic {* auto_tac (MI_fast_css addSIs2 [temp_use (thm "S1Env")]) *})
+  done
+
+lemma Step1_2_2: "|- [HNext rmhist p]_(c p,r p,m p, rmhist!p) & ImpNext p
+         & ~unchanged (e p, c p, r p, m p, rmhist!p) & $S2 rmhist p
+         --> (S3 rmhist p)$ & MClkFwd memCh crCh cst p
+             & unchanged (e p, r p, m p, rmhist!p)"
+  apply (tactic {* action_simp_tac (simpset() addsimps [thm "ImpNext_def"]) []
+    (map temp_elim [thm "S2EnvUnch", thm "S2RPCUnch", thm "S2MemUnch", thm "S2Hist"]) 1 *})
+   apply (tactic {* auto_tac (MI_fast_css addSIs2 [temp_use (thm "S2Clerk"),
+     temp_use (thm "S2Forward")]) *})
+  done
+
+lemma Step1_2_3: "|- [HNext rmhist p]_(c p,r p,m p, rmhist!p) & ImpNext p
+         & ~unchanged (e p, c p, r p, m p, rmhist!p) & $S3 rmhist p
+         --> ((S4 rmhist p)$ & RPCFwd crCh rmCh rst p & unchanged (e p, c p, m p, rmhist!p))
+             | ((S6 rmhist p)$ & RPCFail crCh rmCh rst p & unchanged (e p, c p, m p))"
+  apply (tactic {* action_simp_tac (simpset() addsimps [thm "ImpNext_def"]) []
+    (map temp_elim [thm "S3EnvUnch", thm "S3ClerkUnch", thm "S3MemUnch"]) 1 *})
+  apply (tactic {* action_simp_tac (simpset()) []
+    (thm "squareE" :: map temp_elim [thm "S3RPC", thm "S3Forward", thm "S3Fail"]) 1 *})
+   apply (auto dest!: S3Hist [temp_use])
+  done
+
+lemma Step1_2_4: "|- [HNext rmhist p]_(c p,r p,m p, rmhist!p) & ImpNext p
+              & ~unchanged (e p, c p, r p, m p, rmhist!p)
+              & $S4 rmhist p & (!l. $(MemInv mm l))
+         --> ((S4 rmhist p)$ & Read rmCh mm ires p & unchanged (e p, c p, r p, rmhist!p))
+             | ((S4 rmhist p)$ & (? l. Write rmCh mm ires p l) & unchanged (e p, c p, r p, rmhist!p))
+             | ((S5 rmhist p)$ & MemReturn rmCh ires p & unchanged (e p, c p, r p))"
+  apply (tactic {* action_simp_tac (simpset() addsimps [thm "ImpNext_def"]) []
+    (map temp_elim [thm "S4EnvUnch", thm "S4ClerkUnch", thm "S4RPCUnch"]) 1 *})
+  apply (tactic {* action_simp_tac (simpset() addsimps [thm "RNext_def"]) []
+    (thm "squareE" :: map temp_elim [thm "S4Read", thm "S4Write", thm "S4Return"]) 1 *})
+  apply (auto dest!: S4Hist [temp_use])
+  done
+
+lemma Step1_2_5: "|- [HNext rmhist p]_(c p,r p,m p, rmhist!p) & ImpNext p
+              & ~unchanged (e p, c p, r p, m p, rmhist!p) & $S5 rmhist p
+         --> ((S6 rmhist p)$ & RPCReply crCh rmCh rst p & unchanged (e p, c p, m p))
+             | ((S6 rmhist p)$ & RPCFail crCh rmCh rst p & unchanged (e p, c p, m p))"
+  apply (tactic {* action_simp_tac (simpset() addsimps [thm "ImpNext_def"]) []
+    (map temp_elim [thm "S5EnvUnch", thm "S5ClerkUnch", thm "S5MemUnch", thm "S5Hist"]) 1 *})
+  apply (tactic {* action_simp_tac (simpset()) [] [thm "squareE", temp_elim (thm "S5RPC")] 1 *})
+   apply (tactic {* auto_tac (MI_fast_css addSDs2
+     [temp_use (thm "S5Reply"), temp_use (thm "S5Fail")]) *})
+  done
+
+lemma Step1_2_6: "|- [HNext rmhist p]_(c p,r p,m p, rmhist!p) & ImpNext p
+              & ~unchanged (e p, c p, r p, m p, rmhist!p) & $S6 rmhist p
+         --> ((S1 rmhist p)$ & MClkReply memCh crCh cst p & unchanged (e p, r p, m p))
+             | ((S3 rmhist p)$ & MClkRetry memCh crCh cst p & unchanged (e p,r p,m p,rmhist!p))"
+  apply (tactic {* action_simp_tac (simpset() addsimps [thm "ImpNext_def"]) []
+    (map temp_elim [thm "S6EnvUnch", thm "S6RPCUnch", thm "S6MemUnch"]) 1 *})
+  apply (tactic {* action_simp_tac (simpset()) []
+    (thm "squareE" :: map temp_elim [thm "S6Clerk", thm "S6Retry", thm "S6Reply"]) 1 *})
+     apply (auto dest: S6Hist [temp_use])
+  done
+
+(* --------------------------------------------------------------------------
+   Step 1.3: S1 implies the barred initial condition.
+*)
+
+section "Initialization (Step 1.3)"
+
+lemma Step1_3: "|- S1 rmhist p --> PInit (resbar rmhist) p"
+  by (tactic {* action_simp_tac (simpset () addsimps [thm "resbar_def",
+    thm "PInit_def", thm "S_def", thm "S1_def"]) [] [] 1 *})
+
+(* ----------------------------------------------------------------------
+   Step 1.4: Implementation's next-state relation simulates specification's
+             next-state relation (with appropriate substitutions)
+*)
+
+section "Step simulation (Step 1.4)"
+
+lemma Step1_4_1: "|- ENext p & $S1 rmhist p & (S2 rmhist p)$ & unchanged (c p, r p, m p)
+         --> unchanged (rtrner memCh!p, resbar rmhist!p)"
+  by (tactic {* auto_tac (MI_fast_css addsimps2 [thm "c_def", thm "r_def",
+    thm "m_def", thm "resbar_def"]) *})
+
+lemma Step1_4_2: "|- MClkFwd memCh crCh cst p & $S2 rmhist p & (S3 rmhist p)$
+         & unchanged (e p, r p, m p, rmhist!p)
+         --> unchanged (rtrner memCh!p, resbar rmhist!p)"
+  by (tactic {* action_simp_tac
+    (simpset() addsimps [thm "MClkFwd_def", thm "e_def", thm "r_def", thm "m_def",
+    thm "resbar_def", thm "S_def", thm "S2_def", thm "S3_def"]) [] [] 1 *})
+
+lemma Step1_4_3a: "|- RPCFwd crCh rmCh rst p & $S3 rmhist p & (S4 rmhist p)$
+         & unchanged (e p, c p, m p, rmhist!p)
+         --> unchanged (rtrner memCh!p, resbar rmhist!p)"
+  apply clarsimp
+  apply (drule S3_excl [temp_use] S4_excl [temp_use])+
+  apply (tactic {* action_simp_tac (simpset () addsimps [thm "e_def",
+    thm "c_def", thm "m_def", thm "resbar_def", thm "S_def", thm "S3_def"]) [] [] 1 *})
+  done
+
+lemma Step1_4_3b: "|- RPCFail crCh rmCh rst p & $S3 rmhist p & (S6 rmhist p)$
+         & unchanged (e p, c p, m p)
+         --> MemFail memCh (resbar rmhist) p"
+  apply clarsimp
+  apply (drule S6_excl [temp_use])
+  apply (auto simp: RPCFail_def MemFail_def e_def c_def m_def resbar_def)
+    apply (force simp: S3_def S_def)
+   apply (auto simp: Return_def)
+  done
+
+lemma Step1_4_4a1: "|- $S4 rmhist p & (S4 rmhist p)$ & ReadInner rmCh mm ires p l
+         & unchanged (e p, c p, r p, rmhist!p) & $MemInv mm l
+         --> ReadInner memCh mm (resbar rmhist) p l"
+  apply clarsimp
+  apply (drule S4_excl [temp_use])+
+  apply (tactic {* action_simp_tac (simpset () addsimps [thm "ReadInner_def",
+    thm "GoodRead_def", thm "BadRead_def", thm "e_def", thm "c_def", thm "m_def"]) [] [] 1 *})
+     apply (auto simp: resbar_def)
+       apply (tactic {* ALLGOALS (action_simp_tac
+                (simpset() addsimps [thm "RPCRelayArg_def", thm "MClkRelayArg_def",
+                  thm "S_def", thm "S4_def", thm "RdRequest_def", thm "MemInv_def"])
+                [] [thm "impE", thm "MemValNotAResultE"]) *})
+  done
+
+lemma Step1_4_4a: "|- Read rmCh mm ires p & $S4 rmhist p & (S4 rmhist p)$
+         & unchanged (e p, c p, r p, rmhist!p) & (!l. $(MemInv mm l))
+         --> Read memCh mm (resbar rmhist) p"
+  by (force simp: Read_def elim!: Step1_4_4a1 [temp_use])
+
+lemma Step1_4_4b1: "|- $S4 rmhist p & (S4 rmhist p)$ & WriteInner rmCh mm ires p l v
+         & unchanged (e p, c p, r p, rmhist!p)
+         --> WriteInner memCh mm (resbar rmhist) p l v"
+  apply clarsimp
+  apply (drule S4_excl [temp_use])+
+  apply (tactic {* action_simp_tac (simpset () addsimps
+    [thm "WriteInner_def", thm "GoodWrite_def", thm "BadWrite_def", thm "e_def",
+    thm "c_def", thm "m_def"]) [] [] 1 *})
+     apply (auto simp: resbar_def)
+    apply (tactic {* ALLGOALS (action_simp_tac (simpset () addsimps
+      [thm "RPCRelayArg_def", thm "MClkRelayArg_def", thm "S_def",
+      thm "S4_def", thm "WrRequest_def"]) [] []) *})
+  done
+
+lemma Step1_4_4b: "|- Write rmCh mm ires p l & $S4 rmhist p & (S4 rmhist p)$
+         & unchanged (e p, c p, r p, rmhist!p)
+         --> Write memCh mm (resbar rmhist) p l"
+  by (force simp: Write_def elim!: Step1_4_4b1 [temp_use])
+
+lemma Step1_4_4c: "|- MemReturn rmCh ires p & $S4 rmhist p & (S5 rmhist p)$
+         & unchanged (e p, c p, r p)
+         --> unchanged (rtrner memCh!p, resbar rmhist!p)"
+  apply (tactic {* action_simp_tac (simpset () addsimps [thm "e_def",
+    thm "c_def", thm "r_def", thm "resbar_def"]) [] [] 1 *})
+  apply (drule S4_excl [temp_use] S5_excl [temp_use])+
+  apply (tactic {* auto_tac (MI_fast_css addsimps2 [thm "MemReturn_def", thm "Return_def"]) *})
+  done
+
+lemma Step1_4_5a: "|- RPCReply crCh rmCh rst p & $S5 rmhist p & (S6 rmhist p)$
+         & unchanged (e p, c p, m p)
+         --> unchanged (rtrner memCh!p, resbar rmhist!p)"
+  apply clarsimp
+  apply (drule S5_excl [temp_use] S6_excl [temp_use])+
+  apply (auto simp: e_def c_def m_def resbar_def)
+   apply (auto simp: RPCReply_def Return_def S5_def S_def dest!: MVOKBAnotRF [temp_use])
+  done
+
+lemma Step1_4_5b: "|- RPCFail crCh rmCh rst p & $S5 rmhist p & (S6 rmhist p)$
+         & unchanged (e p, c p, m p)
+         --> MemFail memCh (resbar rmhist) p"
+  apply clarsimp
+  apply (drule S6_excl [temp_use])
+  apply (auto simp: e_def c_def m_def RPCFail_def Return_def MemFail_def resbar_def)
+   apply (auto simp: S5_def S_def)
+  done
+
+lemma Step1_4_6a: "|- MClkReply memCh crCh cst p & $S6 rmhist p & (S1 rmhist p)$
+         & unchanged (e p, r p, m p)
+         --> MemReturn memCh (resbar rmhist) p"
+  apply clarsimp
+  apply (drule S6_excl [temp_use])+
+  apply (tactic {* action_simp_tac (simpset () addsimps [thm "e_def",
+    thm "r_def", thm "m_def", thm "MClkReply_def", thm "MemReturn_def",
+    thm "Return_def", thm "resbar_def"]) [] [] 1 *})
+    apply simp_all (* simplify if-then-else *)
+    apply (tactic {* ALLGOALS (action_simp_tac (simpset () addsimps
+      [thm "MClkReplyVal_def", thm "S6_def", thm "S_def"]) [] [thm "MVOKBARFnotNR"]) *})
+  done
+
+lemma Step1_4_6b: "|- MClkRetry memCh crCh cst p & $S6 rmhist p & (S3 rmhist p)$
+         & unchanged (e p, r p, m p, rmhist!p)
+         --> MemFail memCh (resbar rmhist) p"
+  apply clarsimp
+  apply (drule S3_excl [temp_use])+
+  apply (tactic {* action_simp_tac (simpset () addsimps [thm "e_def", thm "r_def",
+    thm "m_def", thm "MClkRetry_def", thm "MemFail_def", thm "resbar_def"]) [] [] 1 *})
+   apply (auto simp: S6_def S_def)
+  done
+
+lemma S_lemma: "|- unchanged (e p, c p, r p, m p, rmhist!p)
+         --> unchanged (S rmhist ec cc rc cs rs hs1 hs2 p)"
+  by (auto simp: e_def c_def r_def m_def caller_def rtrner_def S_def Calling_def)
+
+lemma Step1_4_7H: "|- unchanged (e p, c p, r p, m p, rmhist!p)
+         --> unchanged (rtrner memCh!p, S1 rmhist p, S2 rmhist p, S3 rmhist p,
+                        S4 rmhist p, S5 rmhist p, S6 rmhist p)"
+  apply clarsimp
+  apply (rule conjI)
+   apply (force simp: c_def)
+  apply (force simp: S1_def S2_def S3_def S4_def S5_def S6_def intro!: S_lemma [temp_use])
+  done
+
+lemma Step1_4_7: "|- unchanged (e p, c p, r p, m p, rmhist!p)
+         --> unchanged (rtrner memCh!p, resbar rmhist!p, S1 rmhist p, S2 rmhist p,
+                        S3 rmhist p, S4 rmhist p, S5 rmhist p, S6 rmhist p)"
+  apply (rule actionI)
+  apply (unfold action_rews)
+  apply (rule impI)
+  apply (frule Step1_4_7H [temp_use])
+  apply (auto simp: e_def c_def r_def m_def rtrner_def resbar_def)
+  done
+
+(* Frequently needed abbreviation: distinguish between idling and non-idling
+   steps of the implementation, and try to solve the idling case by simplification
+*)
+ML {*
+local
+  val actionI = thm "actionI";
+  val action_rews = thms "action_rews";
+  val Step1_4_7 = thm "Step1_4_7";
+in
+fun split_idle_tac simps i =
+    EVERY [TRY (rtac actionI i),
+           case_tac "(s,t) |= unchanged (e p, c p, r p, m p, rmhist!p)" i,
+           rewrite_goals_tac action_rews,
+           forward_tac [temp_use Step1_4_7] i,
+           asm_full_simp_tac (simpset() addsimps simps) i
+          ]
+end
+*}
+(* ----------------------------------------------------------------------
+   Combine steps 1.2 and 1.4 to prove that the implementation satisfies
+   the specification's next-state relation.
+*)
+
+(* Steps that leave all variables unchanged are safe, so I may assume
+   that some variable changes in the proof that a step is safe. *)
+lemma unchanged_safe: "|- (~unchanged (e p, c p, r p, m p, rmhist!p)
+             --> [UNext memCh mm (resbar rmhist) p]_(rtrner memCh!p, resbar rmhist!p))
+         --> [UNext memCh mm (resbar rmhist) p]_(rtrner memCh!p, resbar rmhist!p)"
+  apply (tactic {* split_idle_tac [thm "square_def"] 1 *})
+  apply force
+  done
+(* turn into (unsafe, looping!) introduction rule *)
+lemmas unchanged_safeI = impI [THEN unchanged_safe [action_use], standard]
+
+lemma S1safe: "|- $S1 rmhist p & ImpNext p & [HNext rmhist p]_(c p,r p,m p, rmhist!p)
+         --> [UNext memCh mm (resbar rmhist) p]_(rtrner memCh!p, resbar rmhist!p)"
+  apply clarsimp
+  apply (rule unchanged_safeI)
+  apply (rule idle_squareI)
+  apply (auto dest!: Step1_2_1 [temp_use] Step1_4_1 [temp_use])
+  done
+
+lemma S2safe: "|- $S2 rmhist p & ImpNext p & [HNext rmhist p]_(c p,r p,m p, rmhist!p)
+         --> [UNext memCh mm (resbar rmhist) p]_(rtrner memCh!p, resbar rmhist!p)"
+  apply clarsimp
+  apply (rule unchanged_safeI)
+  apply (rule idle_squareI)
+  apply (auto dest!: Step1_2_2 [temp_use] Step1_4_2 [temp_use])
+  done
+
+lemma S3safe: "|- $S3 rmhist p & ImpNext p & [HNext rmhist p]_(c p,r p,m p, rmhist!p)
+         --> [UNext memCh mm (resbar rmhist) p]_(rtrner memCh!p, resbar rmhist!p)"
+  apply clarsimp
+  apply (rule unchanged_safeI)
+  apply (auto dest!: Step1_2_3 [temp_use])
+  apply (auto simp: square_def UNext_def dest!: Step1_4_3a [temp_use] Step1_4_3b [temp_use])
+  done
+
+lemma S4safe: "|- $S4 rmhist p & ImpNext p & [HNext rmhist p]_(c p,r p,m p, rmhist!p)
+         & (!l. $(MemInv mm l))
+         --> [UNext memCh mm (resbar rmhist) p]_(rtrner memCh!p, resbar rmhist!p)"
+  apply clarsimp
+  apply (rule unchanged_safeI)
+  apply (auto dest!: Step1_2_4 [temp_use])
+     apply (auto simp: square_def UNext_def RNext_def
+       dest!: Step1_4_4a [temp_use] Step1_4_4b [temp_use] Step1_4_4c [temp_use])
+  done
+
+lemma S5safe: "|- $S5 rmhist p & ImpNext p & [HNext rmhist p]_(c p,r p,m p, rmhist!p)
+         --> [UNext memCh mm (resbar rmhist) p]_(rtrner memCh!p, resbar rmhist!p)"
+  apply clarsimp
+  apply (rule unchanged_safeI)
+  apply (auto dest!: Step1_2_5 [temp_use])
+  apply (auto simp: square_def UNext_def dest!: Step1_4_5a [temp_use] Step1_4_5b [temp_use])
+  done
+
+lemma S6safe: "|- $S6 rmhist p & ImpNext p & [HNext rmhist p]_(c p,r p,m p, rmhist!p)
+         --> [UNext memCh mm (resbar rmhist) p]_(rtrner memCh!p, resbar rmhist!p)"
+  apply clarsimp
+  apply (rule unchanged_safeI)
+  apply (auto dest!: Step1_2_6 [temp_use])
+    apply (auto simp: square_def UNext_def RNext_def
+      dest!: Step1_4_6a [temp_use] Step1_4_6b [temp_use])
+  done
+
+(* ----------------------------------------------------------------------
+   Step 1.5: Temporal refinement proof, based on previous steps.
+*)
+
+section "The liveness part"
+
+(* Liveness assertions for the different implementation states, based on the
+   fairness conditions. Prove subgoals of WF1 / SF1 rules as separate lemmas
+   for readability. Reuse action proofs from safety part.
+*)
+
+(* ------------------------------ State S1 ------------------------------ *)
+
+lemma S1_successors: "|- $S1 rmhist p & ImpNext p & [HNext rmhist p]_(c p,r p,m p, rmhist!p)
+         --> (S1 rmhist p)$ | (S2 rmhist p)$"
+  apply (tactic "split_idle_tac [] 1")
+  apply (auto dest!: Step1_2_1 [temp_use])
+  done
+
+(* Show that the implementation can satisfy the high-level fairness requirements
+   by entering the state S1 infinitely often.
+*)
+
+lemma S1_RNextdisabled: "|- S1 rmhist p -->
+         ~Enabled (<RNext memCh mm (resbar rmhist) p>_(rtrner memCh!p, resbar rmhist!p))"
+  apply (tactic {* action_simp_tac (simpset () addsimps [thm "angle_def",
+    thm "S_def", thm "S1_def"]) [notI] [thm "enabledE", temp_elim (thm "Memoryidle")] 1 *})
+  apply force
+  done
+
+lemma S1_Returndisabled: "|- S1 rmhist p -->
+         ~Enabled (<MemReturn memCh (resbar rmhist) p>_(rtrner memCh!p, resbar rmhist!p))"
+  by (tactic {* action_simp_tac (simpset () addsimps [thm "angle_def", thm "MemReturn_def",
+    thm "Return_def", thm "S_def", thm "S1_def"]) [notI] [thm "enabledE"] 1 *})
+
+lemma RNext_fair: "|- []<>S1 rmhist p
+         --> WF(RNext memCh mm (resbar rmhist) p)_(rtrner memCh!p, resbar rmhist!p)"
+  by (auto simp: WF_alt [try_rewrite] intro!: S1_RNextdisabled [temp_use]
+    elim!: STL4E [temp_use] DmdImplE [temp_use])
+
+lemma Return_fair: "|- []<>S1 rmhist p
+         --> WF(MemReturn memCh (resbar rmhist) p)_(rtrner memCh!p, resbar rmhist!p)"
+  by (auto simp: WF_alt [try_rewrite]
+    intro!: S1_Returndisabled [temp_use] elim!: STL4E [temp_use] DmdImplE [temp_use])
+
+(* ------------------------------ State S2 ------------------------------ *)
+
+lemma S2_successors: "|- $S2 rmhist p & ImpNext p & [HNext rmhist p]_(c p,r p,m p, rmhist!p)
+         --> (S2 rmhist p)$ | (S3 rmhist p)$"
+  apply (tactic "split_idle_tac [] 1")
+  apply (auto dest!: Step1_2_2 [temp_use])
+  done
+
+lemma S2MClkFwd_successors: "|- ($S2 rmhist p & ImpNext p & [HNext rmhist p]_(c p,r p,m p, rmhist!p))
+         & <MClkFwd memCh crCh cst p>_(c p)
+         --> (S3 rmhist p)$"
+  by (auto simp: angle_def dest!: Step1_2_2 [temp_use])
+
+lemma S2MClkFwd_enabled: "|- $S2 rmhist p & ImpNext p & [HNext rmhist p]_(c p,r p,m p, rmhist!p)
+         --> $Enabled (<MClkFwd memCh crCh cst p>_(c p))"
+  apply (auto simp: c_def intro!: MClkFwd_ch_enabled [temp_use] MClkFwd_enabled [temp_use])
+     apply (cut_tac MI_base)
+     apply (blast dest: base_pair)
+    apply (simp_all add: S_def S2_def)
+  done
+
+lemma S2_live: "|- [](ImpNext p & [HNext rmhist p]_(c p,r p,m p, rmhist!p))
+         & WF(MClkFwd memCh crCh cst p)_(c p)
+         --> (S2 rmhist p ~> S3 rmhist p)"
+  by (rule WF1 S2_successors S2MClkFwd_successors S2MClkFwd_enabled)+
+
+(* ------------------------------ State S3 ------------------------------ *)
+
+lemma S3_successors: "|- $S3 rmhist p & ImpNext p & [HNext rmhist p]_(c p,r p,m p, rmhist!p)
+         --> (S3 rmhist p)$ | (S4 rmhist p | S6 rmhist p)$"
+  apply (tactic "split_idle_tac [] 1")
+  apply (auto dest!: Step1_2_3 [temp_use])
+  done
+
+lemma S3RPC_successors: "|- ($S3 rmhist p & ImpNext p & [HNext rmhist p]_(c p,r p,m p, rmhist!p))
+         & <RPCNext crCh rmCh rst p>_(r p)
+         --> (S4 rmhist p | S6 rmhist p)$"
+  apply (auto simp: angle_def dest!: Step1_2_3 [temp_use])
+  done
+
+lemma S3RPC_enabled: "|- $S3 rmhist p & ImpNext p & [HNext rmhist p]_(c p,r p,m p, rmhist!p)
+         --> $Enabled (<RPCNext crCh rmCh rst p>_(r p))"
+  apply (auto simp: r_def intro!: RPCFail_Next_enabled [temp_use] RPCFail_enabled [temp_use])
+    apply (cut_tac MI_base)
+    apply (blast dest: base_pair)
+   apply (simp_all add: S_def S3_def)
+  done
+
+lemma S3_live: "|- [](ImpNext p & [HNext rmhist p]_(c p,r p,m p, rmhist!p))
+         & WF(RPCNext crCh rmCh rst p)_(r p)
+         --> (S3 rmhist p ~> S4 rmhist p | S6 rmhist p)"
+  by (rule WF1 S3_successors S3RPC_successors S3RPC_enabled)+
+
+(* ------------- State S4 -------------------------------------------------- *)
+
+lemma S4_successors: "|- $S4 rmhist p & ImpNext p & [HNext rmhist p]_(c p,r p,m p, rmhist!p)
+        & (ALL l. $MemInv mm l)
+        --> (S4 rmhist p)$ | (S5 rmhist p)$"
+  apply (tactic "split_idle_tac [] 1")
+  apply (auto dest!: Step1_2_4 [temp_use])
+  done
+
+(* --------- State S4a: S4 /\ (ires p = NotAResult) ------------------------ *)
+
+lemma S4a_successors: "|- $(S4 rmhist p & ires!p = #NotAResult)
+         & ImpNext p & [HNext rmhist p]_(c p,r p,m p,rmhist!p) & (ALL l. $MemInv mm l)
+         --> (S4 rmhist p & ires!p = #NotAResult)$
+             | ((S4 rmhist p & ires!p ~= #NotAResult) | S5 rmhist p)$"
+  apply (tactic {* split_idle_tac [thm "m_def"] 1 *})
+  apply (auto dest!: Step1_2_4 [temp_use])
+  done
+
+lemma S4aRNext_successors: "|- ($(S4 rmhist p & ires!p = #NotAResult)
+         & ImpNext p & [HNext rmhist p]_(c p,r p,m p,rmhist!p) & (ALL l. $MemInv mm l))
+         & <RNext rmCh mm ires p>_(m p)
+         --> ((S4 rmhist p & ires!p ~= #NotAResult) | S5 rmhist p)$"
+  by (auto simp: angle_def
+    dest!: Step1_2_4 [temp_use] ReadResult [temp_use] WriteResult [temp_use])
+
+lemma S4aRNext_enabled: "|- $(S4 rmhist p & ires!p = #NotAResult)
+         & ImpNext p & [HNext rmhist p]_(c p,r p,m p, rmhist!p) & (ALL l. $MemInv mm l)
+         --> $Enabled (<RNext rmCh mm ires p>_(m p))"
+  apply (auto simp: m_def intro!: RNext_enabled [temp_use])
+   apply (cut_tac MI_base)
+   apply (blast dest: base_pair)
+  apply (simp add: S_def S4_def)
+  done
+
+lemma S4a_live: "|- [](ImpNext p & [HNext rmhist p]_(c p,r p,m p, rmhist!p)
+         & (ALL l. $MemInv mm l)) & WF(RNext rmCh mm ires p)_(m p)
+         --> (S4 rmhist p & ires!p = #NotAResult
+              ~> (S4 rmhist p & ires!p ~= #NotAResult) | S5 rmhist p)"
+  by (rule WF1 S4a_successors S4aRNext_successors S4aRNext_enabled)+
+
+(* ---------- State S4b: S4 /\ (ires p # NotAResult) --------------------------- *)
+
+lemma S4b_successors: "|- $(S4 rmhist p & ires!p ~= #NotAResult)
+         & ImpNext p & [HNext rmhist p]_(c p,r p,m p, rmhist!p) & (ALL l. $MemInv mm l)
+         --> (S4 rmhist p & ires!p ~= #NotAResult)$ | (S5 rmhist p)$"
+  apply (tactic {* split_idle_tac [thm "m_def"] 1 *})
+  apply (auto dest!: WriteResult [temp_use] Step1_2_4 [temp_use] ReadResult [temp_use])
+  done
+
+lemma S4bReturn_successors: "|- ($(S4 rmhist p & ires!p ~= #NotAResult)
+         & ImpNext p & [HNext rmhist p]_(c p,r p,m p, rmhist!p)
+         & (ALL l. $MemInv mm l)) & <MemReturn rmCh ires p>_(m p)
+         --> (S5 rmhist p)$"
+  by (force simp: angle_def dest!: Step1_2_4 [temp_use] dest: ReturnNotReadWrite [temp_use])
+
+lemma S4bReturn_enabled: "|- $(S4 rmhist p & ires!p ~= #NotAResult)
+         & ImpNext p & [HNext rmhist p]_(c p,r p,m p, rmhist!p)
+         & (ALL l. $MemInv mm l)
+         --> $Enabled (<MemReturn rmCh ires p>_(m p))"
+  apply (auto simp: m_def intro!: MemReturn_enabled [temp_use])
+   apply (cut_tac MI_base)
+   apply (blast dest: base_pair)
+  apply (simp add: S_def S4_def)
+  done
+
+lemma S4b_live: "|- [](ImpNext p & [HNext rmhist p]_(c p,r p,m p, rmhist!p) & (!l. $MemInv mm l))
+         & WF(MemReturn rmCh ires p)_(m p)
+         --> (S4 rmhist p & ires!p ~= #NotAResult ~> S5 rmhist p)"
+  by (rule WF1 S4b_successors S4bReturn_successors S4bReturn_enabled)+
+
+(* ------------------------------ State S5 ------------------------------ *)
+
+lemma S5_successors: "|- $S5 rmhist p & ImpNext p & [HNext rmhist p]_(c p,r p,m p, rmhist!p)
+         --> (S5 rmhist p)$ | (S6 rmhist p)$"
+  apply (tactic "split_idle_tac [] 1")
+  apply (auto dest!: Step1_2_5 [temp_use])
+  done
+
+lemma S5RPC_successors: "|- ($S5 rmhist p & ImpNext p & [HNext rmhist p]_(c p,r p,m p, rmhist!p))
+         & <RPCNext crCh rmCh rst p>_(r p)
+         --> (S6 rmhist p)$"
+  by (auto simp: angle_def dest!: Step1_2_5 [temp_use])
+
+lemma S5RPC_enabled: "|- $S5 rmhist p & ImpNext p & [HNext rmhist p]_(c p,r p,m p, rmhist!p)
+         --> $Enabled (<RPCNext crCh rmCh rst p>_(r p))"
+  apply (auto simp: r_def intro!: RPCFail_Next_enabled [temp_use] RPCFail_enabled [temp_use])
+    apply (cut_tac MI_base)
+    apply (blast dest: base_pair)
+   apply (simp_all add: S_def S5_def)
+  done
+
+lemma S5_live: "|- [](ImpNext p & [HNext rmhist p]_(c p,r p,m p, rmhist!p))
+         & WF(RPCNext crCh rmCh rst p)_(r p)
+         --> (S5 rmhist p ~> S6 rmhist p)"
+  by (rule WF1 S5_successors S5RPC_successors S5RPC_enabled)+
+
+(* ------------------------------ State S6 ------------------------------ *)
+
+lemma S6_successors: "|- $S6 rmhist p & ImpNext p & [HNext rmhist p]_(c p,r p,m p, rmhist!p)
+         --> (S1 rmhist p)$ | (S3 rmhist p)$ | (S6 rmhist p)$"
+  apply (tactic "split_idle_tac [] 1")
+  apply (auto dest!: Step1_2_6 [temp_use])
+  done
+
+lemma S6MClkReply_successors:
+  "|- ($S6 rmhist p & ImpNext p & [HNext rmhist p]_(c p,r p,m p, rmhist!p))
+         & <MClkReply memCh crCh cst p>_(c p)
+         --> (S1 rmhist p)$"
+  by (auto simp: angle_def dest!: Step1_2_6 [temp_use] MClkReplyNotRetry [temp_use])
+
+lemma MClkReplyS6:
+  "|- $ImpInv rmhist p & <MClkReply memCh crCh cst p>_(c p) --> $S6 rmhist p"
+  by (tactic {* action_simp_tac (simpset () addsimps [thm "angle_def",
+    thm "MClkReply_def", thm "Return_def", thm "ImpInv_def", thm "S_def",
+    thm "S1_def", thm "S2_def", thm "S3_def", thm "S4_def", thm "S5_def"]) [] [] 1 *})
+
+lemma S6MClkReply_enabled: "|- S6 rmhist p --> Enabled (<MClkReply memCh crCh cst p>_(c p))"
+  apply (auto simp: c_def intro!: MClkReply_enabled [temp_use])
+     apply (cut_tac MI_base)
+     apply (blast dest: base_pair)
+    apply (tactic {* ALLGOALS (action_simp_tac (simpset ()
+      addsimps [thm "S_def", thm "S6_def"]) [] []) *})
+  done
+
+lemma S6_live: "|- [](ImpNext p & [HNext rmhist p]_(c p,r p,m p, rmhist!p) & $(ImpInv rmhist p))
+         & SF(MClkReply memCh crCh cst p)_(c p) & []<>(S6 rmhist p)
+         --> []<>(S1 rmhist p)"
+  apply clarsimp
+  apply (subgoal_tac "sigma |= []<> (<MClkReply memCh crCh cst p>_ (c p))")
+   apply (erule InfiniteEnsures)
+    apply assumption
+   apply (tactic {* action_simp_tac (simpset()) []
+     (map temp_elim [thm "MClkReplyS6", thm "S6MClkReply_successors"]) 1 *})
+  apply (auto simp: SF_def)
+  apply (erule contrapos_np)
+  apply (auto intro!: S6MClkReply_enabled [temp_use] elim!: STL4E [temp_use] DmdImplE [temp_use])
+  done
+
+(* --------------- aggregate leadsto properties----------------------------- *)
+
+lemma S5S6LeadstoS6: "sigma |= S5 rmhist p ~> S6 rmhist p
+      ==> sigma |= (S5 rmhist p | S6 rmhist p) ~> S6 rmhist p"
+  by (auto intro!: LatticeDisjunctionIntro [temp_use] LatticeReflexivity [temp_use])
+
+lemma S4bS5S6LeadstoS6: "[| sigma |= S4 rmhist p & ires!p ~= #NotAResult ~> S5 rmhist p;
+         sigma |= S5 rmhist p ~> S6 rmhist p |]
+      ==> sigma |= (S4 rmhist p & ires!p ~= #NotAResult) | S5 rmhist p | S6 rmhist p
+                    ~> S6 rmhist p"
+  by (auto intro!: LatticeDisjunctionIntro [temp_use]
+    S5S6LeadstoS6 [temp_use] intro: LatticeTransitivity [temp_use])
+
+lemma S4S5S6LeadstoS6: "[| sigma |= S4 rmhist p & ires!p = #NotAResult
+                  ~> (S4 rmhist p & ires!p ~= #NotAResult) | S5 rmhist p;
+         sigma |= S4 rmhist p & ires!p ~= #NotAResult ~> S5 rmhist p;
+         sigma |= S5 rmhist p ~> S6 rmhist p |]
+      ==> sigma |= S4 rmhist p | S5 rmhist p | S6 rmhist p ~> S6 rmhist p"
+  apply (subgoal_tac "sigma |= (S4 rmhist p & ires!p = #NotAResult) |
+    (S4 rmhist p & ires!p ~= #NotAResult) | S5 rmhist p | S6 rmhist p ~> S6 rmhist p")
+   apply (erule_tac G = "PRED ((S4 rmhist p & ires!p = #NotAResult) |
+     (S4 rmhist p & ires!p ~= #NotAResult) | S5 rmhist p | S6 rmhist p)" in
+     LatticeTransitivity [temp_use])
+   apply (force simp: Init_defs intro!: ImplLeadsto_gen [temp_use] necT [temp_use])
+  apply (rule LatticeDisjunctionIntro [temp_use])
+   apply (erule LatticeTransitivity [temp_use])
+   apply (erule LatticeTriangle2 [temp_use])
+   apply assumption
+  apply (auto intro!: S4bS5S6LeadstoS6 [temp_use])
+  done
+
+lemma S3S4S5S6LeadstoS6: "[| sigma |= S3 rmhist p ~> S4 rmhist p | S6 rmhist p;
+         sigma |= S4 rmhist p & ires!p = #NotAResult
+                  ~> (S4 rmhist p & ires!p ~= #NotAResult) | S5 rmhist p;
+         sigma |= S4 rmhist p & ires!p ~= #NotAResult ~> S5 rmhist p;
+         sigma |= S5 rmhist p ~> S6 rmhist p |]
+      ==> sigma |= S3 rmhist p | S4 rmhist p | S5 rmhist p | S6 rmhist p ~> S6 rmhist p"
+  apply (rule LatticeDisjunctionIntro [temp_use])
+   apply (erule LatticeTriangle2 [temp_use])
+   apply (rule S4S5S6LeadstoS6 [THEN LatticeTransitivity [temp_use]])
+      apply (auto intro!: S4S5S6LeadstoS6 [temp_use] necT [temp_use]
+        intro: ImplLeadsto_gen [temp_use] simp: Init_defs)
+  done
+
+lemma S2S3S4S5S6LeadstoS6: "[| sigma |= S2 rmhist p ~> S3 rmhist p;
+         sigma |= S3 rmhist p ~> S4 rmhist p | S6 rmhist p;
+         sigma |= S4 rmhist p & ires!p = #NotAResult
+                  ~> S4 rmhist p & ires!p ~= #NotAResult | S5 rmhist p;
+         sigma |= S4 rmhist p & ires!p ~= #NotAResult ~> S5 rmhist p;
+         sigma |= S5 rmhist p ~> S6 rmhist p |]
+      ==> sigma |= S2 rmhist p | S3 rmhist p | S4 rmhist p | S5 rmhist p | S6 rmhist p
+                   ~> S6 rmhist p"
+  apply (rule LatticeDisjunctionIntro [temp_use])
+   apply (rule LatticeTransitivity [temp_use])
+    prefer 2 apply assumption
+   apply (rule S3S4S5S6LeadstoS6 [THEN LatticeTransitivity [temp_use]])
+       apply (auto intro!: S3S4S5S6LeadstoS6 [temp_use] necT [temp_use]
+         intro: ImplLeadsto_gen [temp_use] simp: Init_defs)
+  done
+
+lemma NotS1LeadstoS6: "[| sigma |= []ImpInv rmhist p;
+         sigma |= S2 rmhist p ~> S3 rmhist p;
+         sigma |= S3 rmhist p ~> S4 rmhist p | S6 rmhist p;
+         sigma |= S4 rmhist p & ires!p = #NotAResult
+                  ~> S4 rmhist p & ires!p ~= #NotAResult | S5 rmhist p;
+         sigma |= S4 rmhist p & ires!p ~= #NotAResult ~> S5 rmhist p;
+         sigma |= S5 rmhist p ~> S6 rmhist p |]
+      ==> sigma |= ~S1 rmhist p ~> S6 rmhist p"
+  apply (rule S2S3S4S5S6LeadstoS6 [THEN LatticeTransitivity [temp_use]])
+       apply assumption+
+  apply (erule INV_leadsto [temp_use])
+  apply (rule ImplLeadsto_gen [temp_use])
+  apply (rule necT [temp_use])
+  apply (auto simp: ImpInv_def Init_defs intro!: necT [temp_use])
+  done
+
+lemma S1Infinite: "[| sigma |= ~S1 rmhist p ~> S6 rmhist p;
+         sigma |= []<>S6 rmhist p --> []<>S1 rmhist p |]
+      ==> sigma |= []<>S1 rmhist p"
+  apply (rule classical)
+  apply (tactic {* asm_lr_simp_tac (simpset() addsimps
+    [temp_use (thm "NotBox"), temp_rewrite (thm "NotDmd")]) 1 *})
+  apply (auto elim!: leadsto_infinite [temp_use] mp dest!: DBImplBD [temp_use])
+  done
+
+section "Refinement proof (step 1.5)"
+
+(* Prove invariants of the implementation:
+   a. memory invariant
+   b. "implementation invariant": always in states S1,...,S6
+*)
+lemma Step1_5_1a: "|- IPImp p --> (ALL l. []$MemInv mm l)"
+  by (auto simp: IPImp_def box_stp_act [temp_use] intro!: MemoryInvariantAll [temp_use])
+
+lemma Step1_5_1b: "|- Init(ImpInit p & HInit rmhist p) & [](ImpNext p)
+         & [][HNext rmhist p]_(c p, r p, m p, rmhist!p) & [](ALL l. $MemInv mm l)
+         --> []ImpInv rmhist p"
+  apply (tactic "inv_tac MI_css 1")
+   apply (auto simp: Init_def ImpInv_def box_stp_act [temp_use]
+     dest!: Step1_1 [temp_use] dest: S1_successors [temp_use] S2_successors [temp_use]
+     S3_successors [temp_use] S4_successors [temp_use] S5_successors [temp_use]
+     S6_successors [temp_use])
+  done
+
+(*** Initialization ***)
+lemma Step1_5_2a: "|- Init(ImpInit p & HInit rmhist p) --> Init(PInit (resbar rmhist) p)"
+  by (auto simp: Init_def intro!: Step1_1 [temp_use] Step1_3  [temp_use])
+
+(*** step simulation ***)
+lemma Step1_5_2b: "|- [](ImpNext p & [HNext rmhist p]_(c p, r p, m p, rmhist!p)
+         & $ImpInv rmhist p & (!l. $MemInv mm l))
+         --> [][UNext memCh mm (resbar rmhist) p]_(rtrner memCh!p, resbar rmhist!p)"
+  by (auto simp: ImpInv_def elim!: STL4E [temp_use]
+    dest!: S1safe [temp_use] S2safe [temp_use] S3safe [temp_use] S4safe [temp_use]
+    S5safe [temp_use] S6safe [temp_use])
+
+(*** Liveness ***)
+lemma GoodImpl: "|- IPImp p & HistP rmhist p
+         -->   Init(ImpInit p & HInit rmhist p)
+             & [](ImpNext p & [HNext rmhist p]_(c p, r p, m p, rmhist!p))
+             & [](ALL l. $MemInv mm l) & []($ImpInv rmhist p)
+             & ImpLive p"
+  apply clarsimp
+    apply (subgoal_tac "sigma |= Init (ImpInit p & HInit rmhist p) & [] (ImpNext p) &
+      [][HNext rmhist p]_ (c p, r p, m p, rmhist!p) & [] (ALL l. $MemInv mm l)")
+   apply (auto simp: split_box_conj [try_rewrite] box_stp_act [try_rewrite]
+       dest!: Step1_5_1b [temp_use])
+      apply (force simp: IPImp_def MClkIPSpec_def RPCIPSpec_def RPSpec_def
+        ImpLive_def c_def r_def m_def)
+      apply (force simp: IPImp_def MClkIPSpec_def RPCIPSpec_def RPSpec_def
+        HistP_def Init_def ImpInit_def)
+    apply (force simp: IPImp_def MClkIPSpec_def RPCIPSpec_def RPSpec_def
+      ImpNext_def c_def r_def m_def split_box_conj [temp_use])
+   apply (force simp: HistP_def)
+  apply (force simp: allT [temp_use] dest!: Step1_5_1a [temp_use])
+  done
+
+(* The implementation is infinitely often in state S1... *)
+lemma Step1_5_3a: "|- [](ImpNext p & [HNext rmhist p]_(c p, r p, m p, rmhist!p))
+         & [](ALL l. $MemInv mm l)
+         & []($ImpInv rmhist p) & ImpLive p
+         --> []<>S1 rmhist p"
+  apply (clarsimp simp: ImpLive_def)
+  apply (rule S1Infinite)
+   apply (force simp: split_box_conj [try_rewrite] box_stp_act [try_rewrite]
+     intro!: NotS1LeadstoS6 [temp_use] S2_live [temp_use] S3_live [temp_use]
+     S4a_live [temp_use] S4b_live [temp_use] S5_live [temp_use])
+  apply (auto simp: split_box_conj [temp_use] intro!: S6_live [temp_use])
+  done
+
+(* ... and therefore satisfies the fairness requirements of the specification *)
+lemma Step1_5_3b: "|- [](ImpNext p & [HNext rmhist p]_(c p, r p, m p, rmhist!p))
+         & [](ALL l. $MemInv mm l) & []($ImpInv rmhist p) & ImpLive p
+         --> WF(RNext memCh mm (resbar rmhist) p)_(rtrner memCh!p, resbar rmhist!p)"
+  by (auto intro!: RNext_fair [temp_use] Step1_5_3a [temp_use])
+
+lemma Step1_5_3c: "|- [](ImpNext p & [HNext rmhist p]_(c p, r p, m p, rmhist!p))
+         & [](ALL l. $MemInv mm l) & []($ImpInv rmhist p) & ImpLive p
+         --> WF(MemReturn memCh (resbar rmhist) p)_(rtrner memCh!p, resbar rmhist!p)"
+  by (auto intro!: Return_fair [temp_use] Step1_5_3a [temp_use])
+
+(* QED step of step 1 *)
+lemma Step1: "|- IPImp p & HistP rmhist p --> UPSpec memCh mm (resbar rmhist) p"
+  by (auto simp: UPSpec_def split_box_conj [temp_use]
+    dest!: GoodImpl [temp_use] intro!: Step1_5_2a [temp_use] Step1_5_2b [temp_use]
+    Step1_5_3b [temp_use] Step1_5_3c [temp_use])
+
+(* ------------------------------ Step 2 ------------------------------ *)
+section "Step 2"
+
+lemma Step2_2a: "|- Write rmCh mm ires p l & ImpNext p
+         & [HNext rmhist p]_(c p, r p, m p, rmhist!p)
+         & $ImpInv rmhist p
+         --> (S4 rmhist p)$ & unchanged (e p, c p, r p, rmhist!p)"
+  apply clarsimp
+  apply (drule WriteS4 [action_use])
+   apply assumption
+  apply (tactic "split_idle_tac [] 1")
+  apply (auto simp: ImpNext_def dest!: S4EnvUnch [temp_use] S4ClerkUnch [temp_use]
+    S4RPCUnch [temp_use])
+     apply (auto simp: square_def dest: S4Write [temp_use])
+  done
+
+lemma Step2_2: "|-   (ALL p. ImpNext p)
+         & (ALL p. [HNext rmhist p]_(c p, r p, m p, rmhist!p))
+         & (ALL p. $ImpInv rmhist p)
+         & [EX q. Write rmCh mm ires q l]_(mm!l)
+         --> [EX q. Write memCh mm (resbar rmhist) q l]_(mm!l)"
+  apply (auto intro!: squareCI elim!: squareE)
+  apply (assumption | rule exI Step1_4_4b [action_use])+
+    apply (force intro!: WriteS4 [temp_use])
+   apply (auto dest!: Step2_2a [temp_use])
+  done
+
+lemma Step2_lemma: "|- [](  (ALL p. ImpNext p)
+            & (ALL p. [HNext rmhist p]_(c p, r p, m p, rmhist!p))
+            & (ALL p. $ImpInv rmhist p)
+            & [EX q. Write rmCh mm ires q l]_(mm!l))
+         --> [][EX q. Write memCh mm (resbar rmhist) q l]_(mm!l)"
+  by (force elim!: STL4E [temp_use] dest!: Step2_2 [temp_use])
+
+lemma Step2: "|- #l : #MemLoc & (ALL p. IPImp p & HistP rmhist p)
+         --> MSpec memCh mm (resbar rmhist) l"
+  apply (auto simp: MSpec_def)
+   apply (force simp: IPImp_def MSpec_def)
+  apply (auto intro!: Step2_lemma [temp_use] simp: split_box_conj [temp_use] all_box [temp_use])
+     prefer 4
+     apply (force simp: IPImp_def MSpec_def)
+    apply (auto simp: split_box_conj [temp_use] elim!: allE dest!: GoodImpl [temp_use])
+  done
+
+(* ----------------------------- Main theorem --------------------------------- *)
+section "Memory implementation"
+
+(* The combination of a legal caller, the memory clerk, the RPC component,
+   and a reliable memory implement the unreliable memory.
+*)
+
+(* Implementation of internal specification by combination of implementation
+   and history variable with explicit refinement mapping
+*)
+lemma Impl_IUSpec: "|- Implementation & Hist rmhist --> IUSpec memCh mm (resbar rmhist)"
+  by (auto simp: IUSpec_def Implementation_def IPImp_def MClkISpec_def
+    RPCISpec_def IRSpec_def Hist_def intro!: Step1 [temp_use] Step2 [temp_use])
+
+(* The main theorem: introduce hiding and eliminate history variable. *)
+lemma Implementation: "|- Implementation --> USpec memCh"
+  apply clarsimp
+  apply (frule History [temp_use])
+  apply (auto simp: USpec_def intro: eexI [temp_use] Impl_IUSpec [temp_use]
+    MI_base [temp_use] elim!: eexE)
+  done
 
 end
