src/HOL/TLA/TLA.thy
@@ -3,12 +3,9 @@
     ID:          $Id$
     Author:      Stephan Merz
     Copyright:   1998 University of Munich
-
-    Theory Name: TLA
-    Logic Image: HOL
-
-The temporal level of TLA.
 *)
+
+header {* The temporal level of TLA *}
 
 theory TLA
 imports Init
@@ -99,6 +96,1108 @@ axioms
               |] ==> G sigma"
   history:    "|- EEX h. Init(h = ha) & [](!x. $h = #x --> h` = hb x)"
 
-ML {* use_legacy_bindings (the_context ()) *}
+
+(* Specialize intensional introduction/elimination rules for temporal formulas *)
+
+lemma tempI: "(!!sigma. sigma |= (F::temporal)) ==> |- F"
+  apply (rule intI)
+  apply (erule meta_spec)
+  done
+
+lemma tempD: "|- (F::temporal) ==> sigma |= F"
+  by (erule intD)
+
+
+(* ======== Functions to "unlift" temporal theorems ====== *)
+
+ML {*
+(* The following functions are specialized versions of the corresponding
+   functions defined in theory Intensional in that they introduce a
+   "world" parameter of type "behavior".
+*)
+local
+  val action_rews = thms "action_rews";
+  val tempD = thm "tempD";
+in
+
+fun temp_unlift th =
+  (rewrite_rule action_rews (th RS tempD)) handle THM _ => action_unlift th;
+
+(* Turn  |- F = G  into meta-level rewrite rule  F == G *)
+val temp_rewrite = int_rewrite
+
+fun temp_use th =
+  case (concl_of th) of
+    Const _ $ (Const ("Intensional.Valid", _) $ _) =>
+            ((flatten (temp_unlift th)) handle THM _ => th)
+  | _ => th;
+
+fun try_rewrite th = temp_rewrite th handle THM _ => temp_use th;
 
 end
+*}
+
+setup {*
+  Attrib.add_attributes [
+    ("temp_unlift", Attrib.no_args (Thm.rule_attribute (K temp_unlift)), ""),
+    ("temp_rewrite", Attrib.no_args (Thm.rule_attribute (K temp_rewrite)), ""),
+    ("temp_use", Attrib.no_args (Thm.rule_attribute (K temp_use)), ""),
+    ("try_rewrite", Attrib.no_args (Thm.rule_attribute (K try_rewrite)), "")]
+*}
+
+(* Update classical reasoner---will be updated once more below! *)
+
+declare tempI [intro!]
+declare tempD [dest]
+ML {*
+val temp_css = (claset(), simpset())
+val temp_cs = op addss temp_css
+*}
+
+(* Modify the functions that add rules to simpsets, classical sets,
+   and clasimpsets in order to accept "lifted" theorems
+*)
+
+(* ------------------------------------------------------------------------- *)
+(***           "Simple temporal logic": only [] and <>                     ***)
+(* ------------------------------------------------------------------------- *)
+section "Simple temporal logic"
+
+(* []~F == []~Init F *)
+lemmas boxNotInit = boxInit [of "LIFT ~F", unfolded Init_simps, standard]
+
+lemma dmdInit: "TEMP <>F == TEMP <> Init F"
+  apply (unfold dmd_def)
+  apply (unfold boxInit [of "LIFT ~F"])
+  apply (simp (no_asm) add: Init_simps)
+  done
+
+lemmas dmdNotInit = dmdInit [of "LIFT ~F", unfolded Init_simps, standard]
+
+(* boxInit and dmdInit cannot be used as rewrites, because they loop.
+   Non-looping instances for state predicates and actions are occasionally useful.
+*)
+lemmas boxInit_stp = boxInit [where 'a = state, standard]
+lemmas boxInit_act = boxInit [where 'a = "state * state", standard]
+lemmas dmdInit_stp = dmdInit [where 'a = state, standard]
+lemmas dmdInit_act = dmdInit [where 'a = "state * state", standard]
+
+(* The symmetric equations can be used to get rid of Init *)
+lemmas boxInitD = boxInit [symmetric]
+lemmas dmdInitD = dmdInit [symmetric]
+lemmas boxNotInitD = boxNotInit [symmetric]
+lemmas dmdNotInitD = dmdNotInit [symmetric]
+
+lemmas Init_simps = Init_simps boxInitD dmdInitD boxNotInitD dmdNotInitD
+
+(* ------------------------ STL2 ------------------------------------------- *)
+lemmas STL2 = reflT
+
+(* The "polymorphic" (generic) variant *)
+lemma STL2_gen: "|- []F --> Init F"
+  apply (unfold boxInit [of F])
+  apply (rule STL2)
+  done
+
+(* see also STL2_pr below: "|- []P --> Init P & Init (P`)" *)
+
+
+(* Dual versions for <> *)
+lemma InitDmd: "|- F --> <> F"
+  apply (unfold dmd_def)
+  apply (auto dest!: STL2 [temp_use])
+  done
+
+lemma InitDmd_gen: "|- Init F --> <>F"
+  apply clarsimp
+  apply (drule InitDmd [temp_use])
+  apply (simp add: dmdInitD)
+  done
+
+
+(* ------------------------ STL3 ------------------------------------------- *)
+lemma STL3: "|- ([][]F) = ([]F)"
+  by (auto elim: transT [temp_use] STL2 [temp_use])
+
+(* corresponding elimination rule introduces double boxes:
+   [| (sigma |= []F); (sigma |= [][]F) ==> PROP W |] ==> PROP W
+*)
+lemmas dup_boxE = STL3 [temp_unlift, THEN iffD2, elim_format]
+lemmas dup_boxD = STL3 [temp_unlift, THEN iffD1, standard]
+
+(* dual versions for <> *)
+lemma DmdDmd: "|- (<><>F) = (<>F)"
+  by (auto simp add: dmd_def [try_rewrite] STL3 [try_rewrite])
+
+lemmas dup_dmdE = DmdDmd [temp_unlift, THEN iffD2, elim_format]
+lemmas dup_dmdD = DmdDmd [temp_unlift, THEN iffD1, standard]
+
+
+(* ------------------------ STL4 ------------------------------------------- *)
+lemma STL4:
+  assumes "|- F --> G"
+  shows "|- []F --> []G"
+  apply clarsimp
+  apply (rule normalT [temp_use])
+   apply (rule assms [THEN necT, temp_use])
+  apply assumption
+  done
+
+(* Unlifted version as an elimination rule *)
+lemma STL4E: "[| sigma |= []F; |- F --> G |] ==> sigma |= []G"
+  by (erule (1) STL4 [temp_use])
+
+lemma STL4_gen: "|- Init F --> Init G ==> |- []F --> []G"
+  apply (drule STL4)
+  apply (simp add: boxInitD)
+  done
+
+lemma STL4E_gen: "[| sigma |= []F; |- Init F --> Init G |] ==> sigma |= []G"
+  by (erule (1) STL4_gen [temp_use])
+
+(* see also STL4Edup below, which allows an auxiliary boxed formula:
+       []A /\ F => G
+     -----------------
+     []A /\ []F => []G
+*)
+
+(* The dual versions for <> *)
+lemma DmdImpl:
+  assumes prem: "|- F --> G"
+  shows "|- <>F --> <>G"
+  apply (unfold dmd_def)
+  apply (fastsimp intro!: prem [temp_use] elim!: STL4E [temp_use])
+  done
+
+lemma DmdImplE: "[| sigma |= <>F; |- F --> G |] ==> sigma |= <>G"
+  by (erule (1) DmdImpl [temp_use])
+
+(* ------------------------ STL5 ------------------------------------------- *)
+lemma STL5: "|- ([]F & []G) = ([](F & G))"
+  apply auto
+  apply (subgoal_tac "sigma |= [] (G --> (F & G))")
+     apply (erule normalT [temp_use])
+     apply (fastsimp elim!: STL4E [temp_use])+
+  done
+
+(* rewrite rule to split conjunctions under boxes *)
+lemmas split_box_conj = STL5 [temp_unlift, symmetric, standard]
+
+
+(* the corresponding elimination rule allows to combine boxes in the hypotheses
+   (NB: F and G must have the same type, i.e., both actions or temporals.)
+   Use "addSE2" etc. if you want to add this to a claset, otherwise it will loop!
+*)
+lemma box_conjE:
+  assumes "sigma |= []F"
+     and "sigma |= []G"
+  and "sigma |= [](F&G) ==> PROP R"
+  shows "PROP R"
+  by (rule assms STL5 [temp_unlift, THEN iffD1] conjI)+
+
+(* Instances of box_conjE for state predicates, actions, and temporals
+   in case the general rule is "too polymorphic".
+*)
+lemmas box_conjE_temp = box_conjE [where 'a = behavior, standard]
+lemmas box_conjE_stp = box_conjE [where 'a = state, standard]
+lemmas box_conjE_act = box_conjE [where 'a = "state * state", standard]
+
+(* Define a tactic that tries to merge all boxes in an antecedent. The definition is
+   a bit kludgy in order to simulate "double elim-resolution".
+*)
+
+lemma box_thin: "[| sigma |= []F; PROP W |] ==> PROP W" .
+
+ML {*
+local
+  val box_conjE = thm "box_conjE";
+  val box_thin = thm "box_thin";
+  val box_conjE_temp = thm "box_conjE_temp";
+  val box_conjE_stp = thm "box_conjE_stp";
+  val box_conjE_act = thm "box_conjE_act";
+in
+
+fun merge_box_tac i =
+   REPEAT_DETERM (EVERY [etac box_conjE i, atac i, etac box_thin i])
+
+fun merge_temp_box_tac i =
+   REPEAT_DETERM (EVERY [etac box_conjE_temp i, atac i,
+                         eres_inst_tac [("'a","behavior")] box_thin i])
+
+fun merge_stp_box_tac i =
+   REPEAT_DETERM (EVERY [etac box_conjE_stp i, atac i,
+                         eres_inst_tac [("'a","state")] box_thin i])
+
+fun merge_act_box_tac i =
+   REPEAT_DETERM (EVERY [etac box_conjE_act i, atac i,
+                         eres_inst_tac [("'a","state * state")] box_thin i])
+
+end
+*}
+
+(* rewrite rule to push universal quantification through box:
+      (sigma |= [](! x. F x)) = (! x. (sigma |= []F x))
+*)
+lemmas all_box = allT [temp_unlift, symmetric, standard]
+
+lemma DmdOr: "|- (<>(F | G)) = (<>F | <>G)"
+  apply (auto simp add: dmd_def split_box_conj [try_rewrite])
+  apply (erule contrapos_np, tactic "merge_box_tac 1",
+    fastsimp elim!: STL4E [temp_use])+
+  done
+
+lemma exT: "|- (EX x. <>(F x)) = (<>(EX x. F x))"
+  by (auto simp: dmd_def Not_Rex [try_rewrite] all_box [try_rewrite])
+
+lemmas ex_dmd = exT [temp_unlift, symmetric, standard]
+
+lemma STL4Edup: "!!sigma. [| sigma |= []A; sigma |= []F; |- F & []A --> G |] ==> sigma |= []G"
+  apply (erule dup_boxE)
+  apply (tactic "merge_box_tac 1")
+  apply (erule STL4E)
+  apply assumption
+  done
+
+lemma DmdImpl2: 
+    "!!sigma. [| sigma |= <>F; sigma |= [](F --> G) |] ==> sigma |= <>G"
+  apply (unfold dmd_def)
+  apply auto
+  apply (erule notE)
+  apply (tactic "merge_box_tac 1")
+  apply (fastsimp elim!: STL4E [temp_use])
+  done
+
+lemma InfImpl:
+  assumes 1: "sigma |= []<>F"
+    and 2: "sigma |= []G"
+    and 3: "|- F & G --> H"
+  shows "sigma |= []<>H"
+  apply (insert 1 2)
+  apply (erule_tac F = G in dup_boxE)
+  apply (tactic "merge_box_tac 1")
+  apply (fastsimp elim!: STL4E [temp_use] DmdImpl2 [temp_use] intro!: 3 [temp_use])
+  done
+
+(* ------------------------ STL6 ------------------------------------------- *)
+(* Used in the proof of STL6, but useful in itself. *)
+lemma BoxDmd: "|- []F & <>G --> <>([]F & G)"
+  apply (unfold dmd_def)
+  apply clarsimp
+  apply (erule dup_boxE)
+  apply (tactic "merge_box_tac 1")
+  apply (erule contrapos_np)
+  apply (fastsimp elim!: STL4E [temp_use])
+  done
+
+(* weaker than BoxDmd, but more polymorphic (and often just right) *)
+lemma BoxDmd_simple: "|- []F & <>G --> <>(F & G)"
+  apply (unfold dmd_def)
+  apply clarsimp
+  apply (tactic "merge_box_tac 1")
+  apply (fastsimp elim!: notE STL4E [temp_use])
+  done
+
+lemma BoxDmd2_simple: "|- []F & <>G --> <>(G & F)"
+  apply (unfold dmd_def)
+  apply clarsimp
+  apply (tactic "merge_box_tac 1")
+  apply (fastsimp elim!: notE STL4E [temp_use])
+  done
+
+lemma DmdImpldup:
+  assumes 1: "sigma |= []A"
+    and 2: "sigma |= <>F"
+    and 3: "|- []A & F --> G"
+  shows "sigma |= <>G"
+  apply (rule 2 [THEN 1 [THEN BoxDmd [temp_use]], THEN DmdImplE])
+  apply (rule 3)
+  done
+
+lemma STL6: "|- <>[]F & <>[]G --> <>[](F & G)"
+  apply (auto simp: STL5 [temp_rewrite, symmetric])
+  apply (drule linT [temp_use])
+   apply assumption
+  apply (erule thin_rl)
+  apply (rule DmdDmd [temp_unlift, THEN iffD1])
+  apply (erule disjE)
+   apply (erule DmdImplE)
+   apply (rule BoxDmd)
+  apply (erule DmdImplE)
+  apply auto
+  apply (drule BoxDmd [temp_use])
+   apply assumption
+  apply (erule thin_rl)
+  apply (fastsimp elim!: DmdImplE [temp_use])
+  done
+
+
+(* ------------------------ True / False ----------------------------------------- *)
+section "Simplification of constants"
+
+lemma BoxConst: "|- ([]#P) = #P"
+  apply (rule tempI)
+  apply (cases P)
+   apply (auto intro!: necT [temp_use] dest: STL2_gen [temp_use] simp: Init_simps)
+  done
+
+lemma DmdConst: "|- (<>#P) = #P"
+  apply (unfold dmd_def)
+  apply (cases P)
+  apply (simp_all add: BoxConst [try_rewrite])
+  done
+
+lemmas temp_simps [temp_rewrite, simp] = BoxConst DmdConst
+
+(* Make these rewrites active by default *)
+ML {*
+val temp_css = temp_css addsimps2 (thms "temp_simps")
+val temp_cs = op addss temp_css
+*}
+
+
+(* ------------------------ Further rewrites ----------------------------------------- *)
+section "Further rewrites"
+
+lemma NotBox: "|- (~[]F) = (<>~F)"
+  by (simp add: dmd_def)
+
+lemma NotDmd: "|- (~<>F) = ([]~F)"
+  by (simp add: dmd_def)
+
+(* These are not declared by default, because they could be harmful,
+   e.g. []F & ~[]F becomes []F & <>~F !! *)
+lemmas more_temp_simps =
+  STL3 [temp_rewrite] DmdDmd [temp_rewrite] NotBox [temp_rewrite] NotDmd [temp_rewrite]
+  NotBox [temp_unlift, THEN eq_reflection]
+  NotDmd [temp_unlift, THEN eq_reflection]
+
+lemma BoxDmdBox: "|- ([]<>[]F) = (<>[]F)"
+  apply (auto dest!: STL2 [temp_use])
+  apply (rule ccontr)
+  apply (subgoal_tac "sigma |= <>[][]F & <>[]~[]F")
+   apply (erule thin_rl)
+   apply auto
+    apply (drule STL6 [temp_use])
+     apply assumption
+    apply simp
+   apply (simp_all add: more_temp_simps)
+  done
+
+lemma DmdBoxDmd: "|- (<>[]<>F) = ([]<>F)"
+  apply (unfold dmd_def)
+  apply (auto simp: BoxDmdBox [unfolded dmd_def, try_rewrite])
+  done
+
+lemmas more_temp_simps = more_temp_simps BoxDmdBox [temp_rewrite] DmdBoxDmd [temp_rewrite]
+
+
+(* ------------------------ Miscellaneous ----------------------------------- *)
+
+lemma BoxOr: "!!sigma. [| sigma |= []F | []G |] ==> sigma |= [](F | G)"
+  by (fastsimp elim!: STL4E [temp_use])
+
+(* "persistently implies infinitely often" *)
+lemma DBImplBD: "|- <>[]F --> []<>F"
+  apply clarsimp
+  apply (rule ccontr)
+  apply (simp add: more_temp_simps)
+  apply (drule STL6 [temp_use])
+   apply assumption
+  apply simp
+  done
+
+lemma BoxDmdDmdBox: "|- []<>F & <>[]G --> []<>(F & G)"
+  apply clarsimp
+  apply (rule ccontr)
+  apply (unfold more_temp_simps)
+  apply (drule STL6 [temp_use])
+   apply assumption
+  apply (subgoal_tac "sigma |= <>[]~F")
+   apply (force simp: dmd_def)
+  apply (fastsimp elim: DmdImplE [temp_use] STL4E [temp_use])
+  done
+
+
+(* ------------------------------------------------------------------------- *)
+(***          TLA-specific theorems: primed formulas                       ***)
+(* ------------------------------------------------------------------------- *)
+section "priming"
+
+(* ------------------------ TLA2 ------------------------------------------- *)
+lemma STL2_pr: "|- []P --> Init P & Init P`"
+  by (fastsimp intro!: STL2_gen [temp_use] primeI [temp_use])
+
+(* Auxiliary lemma allows priming of boxed actions *)
+lemma BoxPrime: "|- []P --> []($P & P$)"
+  apply clarsimp
+  apply (erule dup_boxE)
+  apply (unfold boxInit_act)
+  apply (erule STL4E)
+  apply (auto simp: Init_simps dest!: STL2_pr [temp_use])
+  done
+
+lemma TLA2:
+  assumes "|- $P & P$ --> A"
+  shows "|- []P --> []A"
+  apply clarsimp
+  apply (drule BoxPrime [temp_use])
+  apply (auto simp: Init_stp_act_rev [try_rewrite] intro!: prems [temp_use]
+    elim!: STL4E [temp_use])
+  done
+
+lemma TLA2E: "[| sigma |= []P; |- $P & P$ --> A |] ==> sigma |= []A"
+  by (erule (1) TLA2 [temp_use])
+
+lemma DmdPrime: "|- (<>P`) --> (<>P)"
+  apply (unfold dmd_def)
+  apply (fastsimp elim!: TLA2E [temp_use])
+  done
+
+lemmas PrimeDmd = InitDmd_gen [temp_use, THEN DmdPrime [temp_use], standard]
+
+(* ------------------------ INV1, stable --------------------------------------- *)
+section "stable, invariant"
+
+lemma ind_rule:
+   "[| sigma |= []H; sigma |= Init P; |- H --> (Init P & ~[]F --> Init(P`) & F) |]  
+    ==> sigma |= []F"
+  apply (rule indT [temp_use])
+   apply (erule (2) STL4E)
+  done
+
+lemma box_stp_act: "|- ([]$P) = ([]P)"
+  by (simp add: boxInit_act Init_simps)
+
+lemmas box_stp_actI = box_stp_act [temp_use, THEN iffD2, standard]
+lemmas box_stp_actD = box_stp_act [temp_use, THEN iffD1, standard]
+
+lemmas more_temp_simps = box_stp_act [temp_rewrite] more_temp_simps
+
+lemma INV1: 
+  "|- (Init P) --> (stable P) --> []P"
+  apply (unfold stable_def boxInit_stp boxInit_act)
+  apply clarsimp
+  apply (erule ind_rule)
+   apply (auto simp: Init_simps elim: ind_rule)
+  done
+
+lemma StableT: 
+    "!!P. |- $P & A --> P` ==> |- []A --> stable P"
+  apply (unfold stable_def)
+  apply (fastsimp elim!: STL4E [temp_use])
+  done
+
+lemma Stable: "[| sigma |= []A; |- $P & A --> P` |] ==> sigma |= stable P"
+  by (erule (1) StableT [temp_use])
+
+(* Generalization of INV1 *)
+lemma StableBox: "|- (stable P) --> [](Init P --> []P)"
+  apply (unfold stable_def)
+  apply clarsimp
+  apply (erule dup_boxE)
+  apply (force simp: stable_def elim: STL4E [temp_use] INV1 [temp_use])
+  done
+
+lemma DmdStable: "|- (stable P) & <>P --> <>[]P"
+  apply clarsimp
+  apply (rule DmdImpl2)
+   prefer 2
+   apply (erule StableBox [temp_use])
+  apply (simp add: dmdInitD)
+  done
+
+(* ---------------- (Semi-)automatic invariant tactics ---------------------- *)
+
+ML {*
+local
+  val INV1 = thm "INV1";
+  val Stable = thm "Stable";
+  val Init_stp = thm "Init_stp";
+  val Init_act = thm "Init_act";
+  val squareE = thm "squareE";
+in
+
+(* inv_tac reduces goals of the form ... ==> sigma |= []P *)
+fun inv_tac css = SELECT_GOAL
+     (EVERY [auto_tac css,
+             TRY (merge_box_tac 1),
+             rtac (temp_use INV1) 1, (* fail if the goal is not a box *)
+             TRYALL (etac Stable)]);
+
+(* auto_inv_tac applies inv_tac and then tries to attack the subgoals
+   in simple cases it may be able to handle goals like |- MyProg --> []Inv.
+   In these simple cases the simplifier seems to be more useful than the
+   auto-tactic, which applies too much propositional logic and simplifies
+   too late.
+*)
+fun auto_inv_tac ss = SELECT_GOAL
+    ((inv_tac (claset(),ss) 1) THEN
+     (TRYALL (action_simp_tac (ss addsimps [Init_stp, Init_act]) [] [squareE])));
+end
+*}
+
+lemma unless: "|- []($P --> P` | Q`) --> (stable P) | <>Q"
+  apply (unfold dmd_def)
+  apply (clarsimp dest!: BoxPrime [temp_use])
+  apply (tactic "merge_box_tac 1")
+  apply (erule contrapos_np)
+  apply (fastsimp elim!: Stable [temp_use])
+  done
+
+
+(* --------------------- Recursive expansions --------------------------------------- *)
+section "recursive expansions"
+
+(* Recursive expansions of [] and <> for state predicates *)
+lemma BoxRec: "|- ([]P) = (Init P & []P`)"
+  apply (auto intro!: STL2_gen [temp_use])
+   apply (fastsimp elim!: TLA2E [temp_use])
+  apply (auto simp: stable_def elim!: INV1 [temp_use] STL4E [temp_use])
+  done
+
+lemma DmdRec: "|- (<>P) = (Init P | <>P`)"
+  apply (unfold dmd_def BoxRec [temp_rewrite])
+  apply (auto simp: Init_simps)
+  done
+
+lemma DmdRec2: "!!sigma. [| sigma |= <>P; sigma |= []~P` |] ==> sigma |= Init P"
+  apply (force simp: DmdRec [temp_rewrite] dmd_def)
+  done
+
+lemma InfinitePrime: "|- ([]<>P) = ([]<>P`)"
+  apply auto
+   apply (rule classical)
+   apply (rule DBImplBD [temp_use])
+   apply (subgoal_tac "sigma |= <>[]P")
+    apply (fastsimp elim!: DmdImplE [temp_use] TLA2E [temp_use])
+   apply (subgoal_tac "sigma |= <>[] (<>P & []~P`)")
+    apply (force simp: boxInit_stp [temp_use]
+      elim!: DmdImplE [temp_use] STL4E [temp_use] DmdRec2 [temp_use])
+   apply (force intro!: STL6 [temp_use] simp: more_temp_simps)
+  apply (fastsimp intro: DmdPrime [temp_use] elim!: STL4E [temp_use])
+  done
+
+lemma InfiniteEnsures:
+  "[| sigma |= []N; sigma |= []<>A; |- A & N --> P` |] ==> sigma |= []<>P"
+  apply (unfold InfinitePrime [temp_rewrite])
+  apply (rule InfImpl)
+    apply assumption+
+  done
+
+(* ------------------------ fairness ------------------------------------------- *)
+section "fairness"
+
+(* alternative definitions of fairness *)
+lemma WF_alt: "|- WF(A)_v = ([]<>~Enabled(<A>_v) | []<><A>_v)"
+  apply (unfold WF_def dmd_def)
+  apply fastsimp
+  done
+
+lemma SF_alt: "|- SF(A)_v = (<>[]~Enabled(<A>_v) | []<><A>_v)"
+  apply (unfold SF_def dmd_def)
+  apply fastsimp
+  done
+
+(* theorems to "box" fairness conditions *)
+lemma BoxWFI: "|- WF(A)_v --> []WF(A)_v"
+  by (auto simp: WF_alt [try_rewrite] more_temp_simps intro!: BoxOr [temp_use])
+
+lemma WF_Box: "|- ([]WF(A)_v) = WF(A)_v"
+  by (fastsimp intro!: BoxWFI [temp_use] dest!: STL2 [temp_use])
+
+lemma BoxSFI: "|- SF(A)_v --> []SF(A)_v"
+  by (auto simp: SF_alt [try_rewrite] more_temp_simps intro!: BoxOr [temp_use])
+
+lemma SF_Box: "|- ([]SF(A)_v) = SF(A)_v"
+  by (fastsimp intro!: BoxSFI [temp_use] dest!: STL2 [temp_use])
+
+lemmas more_temp_simps = more_temp_simps WF_Box [temp_rewrite] SF_Box [temp_rewrite]
+
+lemma SFImplWF: "|- SF(A)_v --> WF(A)_v"
+  apply (unfold SF_def WF_def)
+  apply (fastsimp dest!: DBImplBD [temp_use])
+  done
+
+(* A tactic that "boxes" all fairness conditions. Apply more_temp_simps to "unbox". *)
+ML {*
+local
+  val BoxWFI = thm "BoxWFI";
+  val BoxSFI = thm "BoxSFI";
+in 
+val box_fair_tac = SELECT_GOAL (REPEAT (dresolve_tac [BoxWFI,BoxSFI] 1))
+end
+*}
+
+
+(* ------------------------------ leads-to ------------------------------ *)
+
+section "~>"
+
+lemma leadsto_init: "|- (Init F) & (F ~> G) --> <>G"
+  apply (unfold leadsto_def)
+  apply (auto dest!: STL2 [temp_use])
+  done
+
+(* |- F & (F ~> G) --> <>G *)
+lemmas leadsto_init_temp = leadsto_init [where 'a = behavior, unfolded Init_simps, standard]
+
+lemma streett_leadsto: "|- ([]<>Init F --> []<>G) = (<>(F ~> G))"
+  apply (unfold leadsto_def)
+  apply auto
+    apply (simp add: more_temp_simps)
+    apply (fastsimp elim!: DmdImplE [temp_use] STL4E [temp_use])
+   apply (fastsimp intro!: InitDmd [temp_use] elim!: STL4E [temp_use])
+  apply (subgoal_tac "sigma |= []<><>G")
+   apply (simp add: more_temp_simps)
+  apply (drule BoxDmdDmdBox [temp_use])
+   apply assumption
+  apply (fastsimp elim!: DmdImplE [temp_use] STL4E [temp_use])
+  done
+
+lemma leadsto_infinite: "|- []<>F & (F ~> G) --> []<>G"
+  apply clarsimp
+  apply (erule InitDmd [temp_use, THEN streett_leadsto [temp_unlift, THEN iffD2, THEN mp]])
+  apply (simp add: dmdInitD)
+  done
+
+(* In particular, strong fairness is a Streett condition. The following
+   rules are sometimes easier to use than WF2 or SF2 below.
+*)
+lemma leadsto_SF: "|- (Enabled(<A>_v) ~> <A>_v) --> SF(A)_v"
+  apply (unfold SF_def)
+  apply (clarsimp elim!: leadsto_infinite [temp_use])
+  done
+
+lemma leadsto_WF: "|- (Enabled(<A>_v) ~> <A>_v) --> WF(A)_v"
+  by (clarsimp intro!: SFImplWF [temp_use] leadsto_SF [temp_use])
+
+(* introduce an invariant into the proof of a leadsto assertion.
+   []I --> ((P ~> Q)  =  (P /\ I ~> Q))
+*)
+lemma INV_leadsto: "|- []I & (P & I ~> Q) --> (P ~> Q)"
+  apply (unfold leadsto_def)
+  apply clarsimp
+  apply (erule STL4Edup)
+   apply assumption
+  apply (auto simp: Init_simps dest!: STL2_gen [temp_use])
+  done
+
+lemma leadsto_classical: "|- (Init F & []~G ~> G) --> (F ~> G)"
+  apply (unfold leadsto_def dmd_def)
+  apply (force simp: Init_simps elim!: STL4E [temp_use])
+  done
+
+lemma leadsto_false: "|- (F ~> #False) = ([]~F)"
+  apply (unfold leadsto_def)
+  apply (simp add: boxNotInitD)
+  done
+
+lemma leadsto_exists: "|- ((EX x. F x) ~> G) = (ALL x. (F x ~> G))"
+  apply (unfold leadsto_def)
+  apply (auto simp: allT [try_rewrite] Init_simps elim!: STL4E [temp_use])
+  done
+
+(* basic leadsto properties, cf. Unity *)
+
+lemma ImplLeadsto_gen: "|- [](Init F --> Init G) --> (F ~> G)"
+  apply (unfold leadsto_def)
+  apply (auto intro!: InitDmd_gen [temp_use]
+    elim!: STL4E_gen [temp_use] simp: Init_simps)
+  done
+
+lemmas ImplLeadsto = ImplLeadsto_gen [where 'a = behavior and 'b = behavior,
+  unfolded Init_simps, standard]
+
+lemma ImplLeadsto_simple: "!!F G. |- F --> G ==> |- F ~> G"
+  by (auto simp: Init_def intro!: ImplLeadsto_gen [temp_use] necT [temp_use])
+
+lemma EnsuresLeadsto:
+  assumes "|- A & $P --> Q`"
+  shows "|- []A --> (P ~> Q)"
+  apply (unfold leadsto_def)
+  apply (clarsimp elim!: INV_leadsto [temp_use])
+  apply (erule STL4E_gen)
+  apply (auto simp: Init_defs intro!: PrimeDmd [temp_use] assms [temp_use])
+  done
+
+lemma EnsuresLeadsto2: "|- []($P --> Q`) --> (P ~> Q)"
+  apply (unfold leadsto_def)
+  apply clarsimp
+  apply (erule STL4E_gen)
+  apply (auto simp: Init_simps intro!: PrimeDmd [temp_use])
+  done
+
+lemma ensures:
+  assumes 1: "|- $P & N --> P` | Q`"
+    and 2: "|- ($P & N) & A --> Q`"
+  shows "|- []N & []([]P --> <>A) --> (P ~> Q)"
+  apply (unfold leadsto_def)
+  apply clarsimp
+  apply (erule STL4Edup)
+   apply assumption
+  apply clarsimp
+  apply (subgoal_tac "sigmaa |= [] ($P --> P` | Q`) ")
+   apply (drule unless [temp_use])
+   apply (clarsimp dest!: INV1 [temp_use])
+  apply (rule 2 [THEN DmdImpl, temp_use, THEN DmdPrime [temp_use]])
+   apply (force intro!: BoxDmd_simple [temp_use]
+     simp: split_box_conj [try_rewrite] box_stp_act [try_rewrite])
+  apply (force elim: STL4E [temp_use] dest: 1 [temp_use])
+  done
+
+lemma ensures_simple:
+  "[| |- $P & N --> P` | Q`;  
+      |- ($P & N) & A --> Q`  
+   |] ==> |- []N & []<>A --> (P ~> Q)"
+  apply clarsimp
+  apply (erule (2) ensures [temp_use])
+  apply (force elim!: STL4E [temp_use])
+  done
+
+lemma EnsuresInfinite:
+    "[| sigma |= []<>P; sigma |= []A; |- A & $P --> Q` |] ==> sigma |= []<>Q"
+  apply (erule leadsto_infinite [temp_use])
+  apply (erule EnsuresLeadsto [temp_use])
+  apply assumption
+  done
+
+
+(*** Gronning's lattice rules (taken from TLP) ***)
+section "Lattice rules"
+
+lemma LatticeReflexivity: "|- F ~> F"
+  apply (unfold leadsto_def)
+  apply (rule necT InitDmd_gen)+
+  done
+
+lemma LatticeTransitivity: "|- (G ~> H) & (F ~> G) --> (F ~> H)"
+  apply (unfold leadsto_def)
+  apply clarsimp
+  apply (erule dup_boxE) (* [][] (Init G --> H) *)
+  apply (tactic "merge_box_tac 1")
+  apply (clarsimp elim!: STL4E [temp_use])
+  apply (rule dup_dmdD)
+  apply (subgoal_tac "sigmaa |= <>Init G")
+   apply (erule DmdImpl2)
+   apply assumption
+  apply (simp add: dmdInitD)
+  done
+
+lemma LatticeDisjunctionElim1: "|- (F | G ~> H) --> (F ~> H)"
+  apply (unfold leadsto_def)
+  apply (auto simp: Init_simps elim!: STL4E [temp_use])
+  done
+
+lemma LatticeDisjunctionElim2: "|- (F | G ~> H) --> (G ~> H)"
+  apply (unfold leadsto_def)
+  apply (auto simp: Init_simps elim!: STL4E [temp_use])
+  done
+
+lemma LatticeDisjunctionIntro: "|- (F ~> H) & (G ~> H) --> (F | G ~> H)"
+  apply (unfold leadsto_def)
+  apply clarsimp
+  apply (tactic "merge_box_tac 1")
+  apply (auto simp: Init_simps elim!: STL4E [temp_use])
+  done
+
+lemma LatticeDisjunction: "|- (F | G ~> H) = ((F ~> H) & (G ~> H))"
+  by (auto intro: LatticeDisjunctionIntro [temp_use]
+    LatticeDisjunctionElim1 [temp_use]
+    LatticeDisjunctionElim2 [temp_use])
+
+lemma LatticeDiamond: "|- (A ~> B | C) & (B ~> D) & (C ~> D) --> (A ~> D)"
+  apply clarsimp
+  apply (subgoal_tac "sigma |= (B | C) ~> D")
+  apply (erule_tac G = "LIFT (B | C)" in LatticeTransitivity [temp_use])
+   apply (fastsimp intro!: LatticeDisjunctionIntro [temp_use])+
+  done
+
+lemma LatticeTriangle: "|- (A ~> D | B) & (B ~> D) --> (A ~> D)"
+  apply clarsimp
+  apply (subgoal_tac "sigma |= (D | B) ~> D")
+   apply (erule_tac G = "LIFT (D | B)" in LatticeTransitivity [temp_use])
+  apply assumption
+  apply (auto intro: LatticeDisjunctionIntro [temp_use] LatticeReflexivity [temp_use])
+  done
+
+lemma LatticeTriangle2: "|- (A ~> B | D) & (B ~> D) --> (A ~> D)"
+  apply clarsimp
+  apply (subgoal_tac "sigma |= B | D ~> D")
+   apply (erule_tac G = "LIFT (B | D)" in LatticeTransitivity [temp_use])
+   apply assumption
+  apply (auto intro: LatticeDisjunctionIntro [temp_use] LatticeReflexivity [temp_use])
+  done
+
+(*** Lamport's fairness rules ***)
+section "Fairness rules"
+
+lemma WF1:
+  "[| |- $P & N  --> P` | Q`;    
+      |- ($P & N) & <A>_v --> Q`;    
+      |- $P & N --> $(Enabled(<A>_v)) |]    
+  ==> |- []N & WF(A)_v --> (P ~> Q)"
+  apply (clarsimp dest!: BoxWFI [temp_use])
+  apply (erule (2) ensures [temp_use])
+  apply (erule (1) STL4Edup)
+  apply (clarsimp simp: WF_def)
+  apply (rule STL2 [temp_use])
+  apply (clarsimp elim!: mp intro!: InitDmd [temp_use])
+  apply (erule STL4 [temp_use, THEN box_stp_actD [temp_use]])
+  apply (simp add: split_box_conj box_stp_actI)
+  done
+
+(* Sometimes easier to use; designed for action B rather than state predicate Q *)
+lemma WF_leadsto:
+  assumes 1: "|- N & $P --> $Enabled (<A>_v)"
+    and 2: "|- N & <A>_v --> B"
+    and 3: "|- [](N & [~A]_v) --> stable P"
+  shows "|- []N & WF(A)_v --> (P ~> B)"
+  apply (unfold leadsto_def)
+  apply (clarsimp dest!: BoxWFI [temp_use])
+  apply (erule (1) STL4Edup)
+  apply clarsimp
+  apply (rule 2 [THEN DmdImpl, temp_use])
+  apply (rule BoxDmd_simple [temp_use])
+   apply assumption
+  apply (rule classical)
+  apply (rule STL2 [temp_use])
+  apply (clarsimp simp: WF_def elim!: mp intro!: InitDmd [temp_use])
+  apply (rule 1 [THEN STL4, temp_use, THEN box_stp_actD])
+  apply (simp (no_asm_simp) add: split_box_conj [try_rewrite] box_stp_act [try_rewrite])
+  apply (erule INV1 [temp_use])
+  apply (rule 3 [temp_use])
+  apply (simp add: split_box_conj [try_rewrite] NotDmd [temp_use] not_angle [try_rewrite])
+  done
+
+lemma SF1:
+  "[| |- $P & N  --> P` | Q`;    
+      |- ($P & N) & <A>_v --> Q`;    
+      |- []P & []N & []F --> <>Enabled(<A>_v) |]    
+  ==> |- []N & SF(A)_v & []F --> (P ~> Q)"
+  apply (clarsimp dest!: BoxSFI [temp_use])
+  apply (erule (2) ensures [temp_use])
+  apply (erule_tac F = F in dup_boxE)
+  apply (tactic "merge_temp_box_tac 1")
+  apply (erule STL4Edup)
+  apply assumption
+  apply (clarsimp simp: SF_def)
+  apply (rule STL2 [temp_use])
+  apply (erule mp)
+  apply (erule STL4 [temp_use])
+  apply (simp add: split_box_conj [try_rewrite] STL3 [try_rewrite])
+  done
+
+lemma WF2:
+  assumes 1: "|- N & <B>_f --> <M>_g"
+    and 2: "|- $P & P` & <N & A>_f --> B"
+    and 3: "|- P & Enabled(<M>_g) --> Enabled(<A>_f)"
+    and 4: "|- [](N & [~B]_f) & WF(A)_f & []F & <>[]Enabled(<M>_g) --> <>[]P"
+  shows "|- []N & WF(A)_f & []F --> WF(M)_g"
+  apply (clarsimp dest!: BoxWFI [temp_use] BoxDmdBox [temp_use, THEN iffD2]
+    simp: WF_def [where A = M])
+  apply (erule_tac F = F in dup_boxE)
+  apply (tactic "merge_temp_box_tac 1")
+  apply (erule STL4Edup)
+   apply assumption
+  apply (clarsimp intro!: BoxDmd_simple [temp_use, THEN 1 [THEN DmdImpl, temp_use]])
+  apply (rule classical)
+  apply (subgoal_tac "sigmaa |= <> (($P & P` & N) & <A>_f)")
+   apply (force simp: angle_def intro!: 2 [temp_use] elim!: DmdImplE [temp_use])
+  apply (rule BoxDmd_simple [THEN DmdImpl, unfolded DmdDmd [temp_rewrite], temp_use])
+  apply (simp add: NotDmd [temp_use] not_angle [try_rewrite])
+  apply (tactic "merge_act_box_tac 1")
+  apply (frule 4 [temp_use])
+     apply assumption+
+  apply (drule STL6 [temp_use])
+   apply assumption
+  apply (erule_tac V = "sigmaa |= <>[]P" in thin_rl)
+  apply (erule_tac V = "sigmaa |= []F" in thin_rl)
+  apply (drule BoxWFI [temp_use])
+  apply (erule_tac F = "ACT N & [~B]_f" in dup_boxE)
+  apply (tactic "merge_temp_box_tac 1")
+  apply (erule DmdImpldup)
+   apply assumption
+  apply (auto simp: split_box_conj [try_rewrite] STL3 [try_rewrite]
+    WF_Box [try_rewrite] box_stp_act [try_rewrite])
+   apply (force elim!: TLA2E [where P = P, temp_use])
+  apply (rule STL2 [temp_use])
+  apply (force simp: WF_def split_box_conj [try_rewrite]
+    elim!: mp intro!: InitDmd [temp_use] 3 [THEN STL4, temp_use])
+  done
+
+lemma SF2:
+  assumes 1: "|- N & <B>_f --> <M>_g"
+    and 2: "|- $P & P` & <N & A>_f --> B"
+    and 3: "|- P & Enabled(<M>_g) --> Enabled(<A>_f)"
+    and 4: "|- [](N & [~B]_f) & SF(A)_f & []F & []<>Enabled(<M>_g) --> <>[]P"
+  shows "|- []N & SF(A)_f & []F --> SF(M)_g"
+  apply (clarsimp dest!: BoxSFI [temp_use] simp: 2 [try_rewrite] SF_def [where A = M])
+  apply (erule_tac F = F in dup_boxE)
+  apply (erule_tac F = "TEMP <>Enabled (<M>_g) " in dup_boxE)
+  apply (tactic "merge_temp_box_tac 1")
+  apply (erule STL4Edup)
+   apply assumption
+  apply (clarsimp intro!: BoxDmd_simple [temp_use, THEN 1 [THEN DmdImpl, temp_use]])
+  apply (rule classical)
+  apply (subgoal_tac "sigmaa |= <> (($P & P` & N) & <A>_f)")
+   apply (force simp: angle_def intro!: 2 [temp_use] elim!: DmdImplE [temp_use])
+  apply (rule BoxDmd_simple [THEN DmdImpl, unfolded DmdDmd [temp_rewrite], temp_use])
+  apply (simp add: NotDmd [temp_use] not_angle [try_rewrite])
+  apply (tactic "merge_act_box_tac 1")
+  apply (frule 4 [temp_use])
+     apply assumption+
+  apply (erule_tac V = "sigmaa |= []F" in thin_rl)
+  apply (drule BoxSFI [temp_use])
+  apply (erule_tac F = "TEMP <>Enabled (<M>_g)" in dup_boxE)
+  apply (erule_tac F = "ACT N & [~B]_f" in dup_boxE)
+  apply (tactic "merge_temp_box_tac 1")
+  apply (erule DmdImpldup)
+   apply assumption
+  apply (auto simp: split_box_conj [try_rewrite] STL3 [try_rewrite]
+    SF_Box [try_rewrite] box_stp_act [try_rewrite])
+   apply (force elim!: TLA2E [where P = P, temp_use])
+  apply (rule STL2 [temp_use])
+  apply (force simp: SF_def split_box_conj [try_rewrite]
+    elim!: mp InfImpl [temp_use] intro!: 3 [temp_use])
+  done
+
+(* ------------------------------------------------------------------------- *)
+(***           Liveness proofs by well-founded orderings                   ***)
+(* ------------------------------------------------------------------------- *)
+section "Well-founded orderings"
+
+lemma wf_leadsto:
+  assumes 1: "wf r"
+    and 2: "!!x. sigma |= F x ~> (G | (EX y. #((y,x):r) & F y))    "
+  shows "sigma |= F x ~> G"
+  apply (rule 1 [THEN wf_induct])
+  apply (rule LatticeTriangle [temp_use])
+   apply (rule 2)
+  apply (auto simp: leadsto_exists [try_rewrite])
+  apply (case_tac "(y,x) :r")
+   apply force
+  apply (force simp: leadsto_def Init_simps intro!: necT [temp_use])
+  done
+
+(* If r is well-founded, state function v cannot decrease forever *)
+lemma wf_not_box_decrease: "!!r. wf r ==> |- [][ (v`, $v) : #r ]_v --> <>[][#False]_v"
+  apply clarsimp
+  apply (rule ccontr)
+  apply (subgoal_tac "sigma |= (EX x. v=#x) ~> #False")
+   apply (drule leadsto_false [temp_use, THEN iffD1, THEN STL2_gen [temp_use]])
+   apply (force simp: Init_defs)
+  apply (clarsimp simp: leadsto_exists [try_rewrite] not_square [try_rewrite] more_temp_simps)
+  apply (erule wf_leadsto)
+  apply (rule ensures_simple [temp_use])
+     apply (tactic "TRYALL atac")
+   apply (auto simp: square_def angle_def)
+  done
+
+(* "wf r  ==>  |- <>[][ (v`, $v) : #r ]_v --> <>[][#False]_v" *)
+lemmas wf_not_dmd_box_decrease =
+  wf_not_box_decrease [THEN DmdImpl, unfolded more_temp_simps, standard]
+
+(* If there are infinitely many steps where v decreases, then there
+   have to be infinitely many non-stuttering steps where v doesn't decrease.
+*)
+lemma wf_box_dmd_decrease:
+  assumes 1: "wf r"
+  shows "|- []<>((v`, $v) : #r) --> []<><(v`, $v) ~: #r>_v"
+  apply clarsimp
+  apply (rule ccontr)
+  apply (simp add: not_angle [try_rewrite] more_temp_simps)
+  apply (drule 1 [THEN wf_not_dmd_box_decrease [temp_use]])
+  apply (drule BoxDmdDmdBox [temp_use])
+   apply assumption
+  apply (subgoal_tac "sigma |= []<> ((#False) ::action)")
+   apply force
+  apply (erule STL4E)
+  apply (rule DmdImpl)
+  apply (force intro: 1 [THEN wf_irrefl, temp_use])
+  done
+
+(* In particular, for natural numbers, if n decreases infinitely often
+   then it has to increase infinitely often.
+*)
+lemma nat_box_dmd_decrease: "!!n::nat stfun. |- []<>(n` < $n) --> []<>($n < n`)"
+  apply clarsimp
+  apply (subgoal_tac "sigma |= []<><~ ((n`,$n) : #less_than) >_n")
+   apply (erule thin_rl)
+   apply (erule STL4E)
+   apply (rule DmdImpl)
+   apply (clarsimp simp: angle_def [try_rewrite])
+  apply (rule wf_box_dmd_decrease [temp_use])
+   apply (auto elim!: STL4E [temp_use] DmdImplE [temp_use])
+  done
+
+
+(* ------------------------------------------------------------------------- *)
+(***           Flexible quantification over state variables                ***)
+(* ------------------------------------------------------------------------- *)
+section "Flexible quantification"
+
+lemma aallI:
+  assumes 1: "basevars vs"
+    and 2: "(!!x. basevars (x,vs) ==> sigma |= F x)"
+  shows "sigma |= (AALL x. F x)"
+  by (auto simp: aall_def elim!: eexE [temp_use] intro!: 1 dest!: 2 [temp_use])
+
+lemma aallE: "|- (AALL x. F x) --> F x"
+  apply (unfold aall_def)
+  apply clarsimp
+  apply (erule contrapos_np)
+  apply (force intro!: eexI [temp_use])
+  done
+
+(* monotonicity of quantification *)
+lemma eex_mono:
+  assumes 1: "sigma |= EEX x. F x"
+    and 2: "!!x. sigma |= F x --> G x"
+  shows "sigma |= EEX x. G x"
+  apply (rule unit_base [THEN 1 [THEN eexE]])
+  apply (rule eexI [temp_use])
+  apply (erule 2 [unfolded intensional_rews, THEN mp])
+  done
+
+lemma aall_mono:
+  assumes 1: "sigma |= AALL x. F(x)"
+    and 2: "!!x. sigma |= F(x) --> G(x)"
+  shows "sigma |= AALL x. G(x)"
+  apply (rule unit_base [THEN aallI])
+  apply (rule 2 [unfolded intensional_rews, THEN mp])
+  apply (rule 1 [THEN aallE [temp_use]])
+  done
+
+(* Derived history introduction rule *)
+lemma historyI:
+  assumes 1: "sigma |= Init I"
+    and 2: "sigma |= []N"
+    and 3: "basevars vs"
+    and 4: "!!h. basevars(h,vs) ==> |- I & h = ha --> HI h"
+    and 5: "!!h s t. [| basevars(h,vs); N (s,t); h t = hb (h s) (s,t) |] ==> HN h (s,t)"
+  shows "sigma |= EEX h. Init (HI h) & [](HN h)"
+  apply (rule history [temp_use, THEN eexE])
+  apply (rule 3)
+  apply (rule eexI [temp_use])
+  apply clarsimp
+  apply (rule conjI)
+   prefer 2
+   apply (insert 2)
+   apply (tactic "merge_box_tac 1")
+   apply (force elim!: STL4E [temp_use] 5 [temp_use])
+  apply (insert 1)
+  apply (force simp: Init_defs elim!: 4 [temp_use])
+  done
+
+(* ----------------------------------------------------------------------
+   example of a history variable: existence of a clock
+*)
+
+lemma "|- EEX h. Init(h = #True) & [](h` = (~$h))"
+  apply (rule tempI)
+  apply (rule historyI)
+  apply (force simp: Init_defs intro!: unit_base [temp_use] necT [temp_use])+
+  done
+
+end
+
