src/HOL/TLA/Inc/Inc.thy
@@ -3,9 +3,6 @@
     ID:          $Id$
     Author:      Stephan Merz
     Copyright:   1997 University of Munich
-
-    Theory Name: Inc
-    Logic Image: TLA    
 *)
 
 header {* Lamport's "increment" example *}
@@ -85,6 +82,234 @@ axioms
   PsiInv3_def:  "PsiInv3  == PRED sem = # 0 & pc2 = #a & (pc1 = #b | pc1 = #g)"
   PsiInv_def:   "PsiInv   == PRED (PsiInv1 | PsiInv2 | PsiInv3)"
 
-ML {* use_legacy_bindings (the_context ()) *}
+
+lemmas PsiInv_defs = PsiInv_def PsiInv1_def PsiInv2_def PsiInv3_def
+lemmas Psi_defs = Psi_def InitPsi_def N1_def N2_def alpha1_def alpha2_def
+  beta1_def beta2_def gamma1_def gamma2_def
+
+
+(*** Invariant proof for Psi: "manual" proof proves individual lemmas ***)
+
+lemma PsiInv_Init: "|- InitPsi --> PsiInv"
+  by (auto simp: InitPsi_def PsiInv_defs)
+
+lemma PsiInv_alpha1: "|- alpha1 & $PsiInv --> PsiInv$"
+  by (auto simp: alpha1_def PsiInv_defs)
+
+lemma PsiInv_alpha2: "|- alpha2 & $PsiInv --> PsiInv$"
+  by (auto simp: alpha2_def PsiInv_defs)
+
+lemma PsiInv_beta1: "|- beta1 & $PsiInv --> PsiInv$"
+  by (auto simp: beta1_def PsiInv_defs)
+
+lemma PsiInv_beta2: "|- beta2 & $PsiInv --> PsiInv$"
+  by (auto simp: beta2_def PsiInv_defs)
+
+lemma PsiInv_gamma1: "|- gamma1 & $PsiInv --> PsiInv$"
+  by (auto simp: gamma1_def PsiInv_defs)
+
+lemma PsiInv_gamma2: "|- gamma2 & $PsiInv --> PsiInv$"
+  by (auto simp: gamma2_def PsiInv_defs)
+
+lemma PsiInv_stutter: "|- unchanged (x,y,sem,pc1,pc2) & $PsiInv --> PsiInv$"
+  by (auto simp: PsiInv_defs)
+
+lemma PsiInv: "|- Psi --> []PsiInv"
+  apply (tactic {* inv_tac (clasimpset () addsimps2 [thm "Psi_def"]) 1 *})
+   apply (force simp: PsiInv_Init [try_rewrite] Init_def)
+  apply (auto intro: PsiInv_alpha1 [try_rewrite] PsiInv_alpha2 [try_rewrite]
+    PsiInv_beta1 [try_rewrite] PsiInv_beta2 [try_rewrite] PsiInv_gamma1 [try_rewrite]
+    PsiInv_gamma2 [try_rewrite] PsiInv_stutter [try_rewrite]
+    simp add: square_def N1_def N2_def)
+  done
+
+(* Automatic proof works too, but it make take a while on a slow machine.
+   More realistic examples require user guidance anyway.
+*)
+
+lemma "|- Psi --> []PsiInv"
+  by (tactic {* auto_inv_tac (simpset() addsimps (thms "PsiInv_defs" @ thms "Psi_defs")) 1 *})
+
+
+(**** Step simulation ****)
+
+lemma Init_sim: "|- Psi --> Init InitPhi"
+  by (auto simp: InitPhi_def Psi_def InitPsi_def Init_def)
+
+lemma Step_sim: "|- Psi --> [][M1 | M2]_(x,y)"
+  by (auto simp: square_def M1_def M2_def Psi_defs elim!: STL4E [temp_use])
+
+
+(**** Proof of fairness ****)
+
+(*
+   The goal is to prove Fair_M1 far below, which asserts
+         |- Psi --> WF(M1)_(x,y)
+   (the other fairness condition is symmetrical).
+
+   The strategy is to use WF2 (with beta1 as the helpful action). Proving its
+   temporal premise needs two auxiliary lemmas:
+   1. Stuck_at_b: control can only proceed at pc1 = b by executing beta1
+   2. N1_live: the first component will eventually reach b
+
+   Lemma 1 is easy, lemma 2 relies on the invariant, the strong fairness
+   of the semaphore, and needs auxiliary lemmas that ensure that the second
+   component will eventually release the semaphore. Most of the proofs of
+   the auxiliary lemmas are very similar.
+*)
+
+lemma Stuck_at_b: "|- [][(N1 | N2) & ~ beta1]_(x,y,sem,pc1,pc2) --> stable(pc1 = #b)"
+  by (auto elim!: Stable squareE simp: Psi_defs)
+
+lemma N1_enabled_at_g: "|- pc1 = #g --> Enabled (<N1>_(x,y,sem,pc1,pc2))"
+  apply clarsimp
+  apply (rule_tac F = gamma1 in enabled_mono)
+   apply (tactic {* enabled_tac (thm "Inc_base") 1 *})
+  apply (force simp: gamma1_def)
+  apply (force simp: angle_def gamma1_def N1_def)
+  done
+
+lemma g1_leadsto_a1:
+  "|- [][(N1 | N2) & ~beta1]_(x,y,sem,pc1,pc2) & SF(N1)_(x,y,sem,pc1,pc2) & []#True  
+    --> (pc1 = #g ~> pc1 = #a)"
+  apply (rule SF1)
+    apply (tactic
+      {* action_simp_tac (simpset () addsimps (thms "Psi_defs")) [] [thm "squareE"] 1 *})
+   apply (tactic
+      {* action_simp_tac (simpset () addsimps (thm "angle_def" :: thms "Psi_defs")) [] [] 1 *})
+  (* reduce |- []A --> <>Enabled B  to  |- A --> Enabled B *)
+  apply (auto intro!: InitDmd_gen [temp_use] N1_enabled_at_g [temp_use]
+    dest!: STL2_gen [temp_use] simp: Init_def)
+  done
+
+(* symmetrical for N2, and similar for beta2 *)
+lemma N2_enabled_at_g: "|- pc2 = #g --> Enabled (<N2>_(x,y,sem,pc1,pc2))"
+  apply clarsimp
+  apply (rule_tac F = gamma2 in enabled_mono)
+  apply (tactic {* enabled_tac (thm "Inc_base") 1 *})
+   apply (force simp: gamma2_def)
+  apply (force simp: angle_def gamma2_def N2_def)
+  done
+
+lemma g2_leadsto_a2:
+  "|- [][(N1 | N2) & ~beta1]_(x,y,sem,pc1,pc2) & SF(N2)_(x,y,sem,pc1,pc2) & []#True  
+    --> (pc2 = #g ~> pc2 = #a)"
+  apply (rule SF1)
+  apply (tactic {* action_simp_tac (simpset () addsimps (thms "Psi_defs")) [] [thm "squareE"] 1 *})
+  apply (tactic {* action_simp_tac (simpset () addsimps (thm "angle_def" :: thms "Psi_defs"))
+    [] [] 1 *})
+  apply (auto intro!: InitDmd_gen [temp_use] N2_enabled_at_g [temp_use]
+    dest!: STL2_gen [temp_use] simp add: Init_def)
+  done
+
+lemma N2_enabled_at_b: "|- pc2 = #b --> Enabled (<N2>_(x,y,sem,pc1,pc2))"
+  apply clarsimp
+  apply (rule_tac F = beta2 in enabled_mono)
+   apply (tactic {* enabled_tac (thm "Inc_base") 1 *})
+   apply (force simp: beta2_def)
+  apply (force simp: angle_def beta2_def N2_def)
+  done
+
+lemma b2_leadsto_g2:
+  "|- [][(N1 | N2) & ~beta1]_(x,y,sem,pc1,pc2) & SF(N2)_(x,y,sem,pc1,pc2) & []#True  
+    --> (pc2 = #b ~> pc2 = #g)"
+  apply (rule SF1)
+    apply (tactic
+      {* action_simp_tac (simpset () addsimps (thms "Psi_defs")) [] [thm "squareE"] 1 *})
+   apply (tactic
+     {* action_simp_tac (simpset () addsimps (thm "angle_def" :: thms "Psi_defs")) [] [] 1 *})
+  apply (auto intro!: InitDmd_gen [temp_use] N2_enabled_at_b [temp_use]
+    dest!: STL2_gen [temp_use] simp: Init_def)
+  done
+
+(* Combine above lemmas: the second component will eventually reach pc2 = a *)
+lemma N2_leadsto_a:
+  "|- [][(N1 | N2) & ~beta1]_(x,y,sem,pc1,pc2) & SF(N2)_(x,y,sem,pc1,pc2) & []#True  
+    --> (pc2 = #a | pc2 = #b | pc2 = #g ~> pc2 = #a)"
+  apply (auto intro!: LatticeDisjunctionIntro [temp_use])
+    apply (rule LatticeReflexivity [temp_use])
+   apply (rule LatticeTransitivity [temp_use])
+  apply (auto intro!: b2_leadsto_g2 [temp_use] g2_leadsto_a2 [temp_use])
+  done
+
+(* Get rid of disjunction on the left-hand side of ~> above. *)
+lemma N2_live:
+  "|- [][(N1 | N2) & ~beta1]_(x,y,sem,pc1,pc2) & SF(N2)_(x,y,sem,pc1,pc2)  
+    --> <>(pc2 = #a)"
+  apply (auto simp: Init_defs intro!: N2_leadsto_a [temp_use, THEN [2] leadsto_init [temp_use]])
+  apply (case_tac "pc2 (st1 sigma)")
+    apply auto
+  done
+
+(* Now prove that the first component will eventually reach pc1 = b from pc1 = a *)
+
+lemma N1_enabled_at_both_a:
+  "|- pc2 = #a & (PsiInv & pc1 = #a) --> Enabled (<N1>_(x,y,sem,pc1,pc2))"
+  apply clarsimp
+  apply (rule_tac F = alpha1 in enabled_mono)
+  apply (tactic {* enabled_tac (thm "Inc_base") 1 *})
+   apply (force simp: alpha1_def PsiInv_defs)
+  apply (force simp: angle_def alpha1_def N1_def)
+  done
+
+lemma a1_leadsto_b1:
+  "|- []($PsiInv & [(N1 | N2) & ~beta1]_(x,y,sem,pc1,pc2))       
+         & SF(N1)_(x,y,sem,pc1,pc2) & [] SF(N2)_(x,y,sem,pc1,pc2)   
+         --> (pc1 = #a ~> pc1 = #b)"
+  apply (rule SF1)
+  apply (tactic {* action_simp_tac (simpset () addsimps thms "Psi_defs") [] [thm "squareE"] 1 *})
+  apply (tactic
+    {* action_simp_tac (simpset () addsimps (thm "angle_def" :: thms "Psi_defs")) [] [] 1 *})
+  apply (clarsimp intro!: N1_enabled_at_both_a [THEN DmdImpl [temp_use]])
+  apply (auto intro!: BoxDmd2_simple [temp_use] N2_live [temp_use]
+    simp: split_box_conj more_temp_simps)
+  done
+
+(* Combine the leadsto properties for N1: it will arrive at pc1 = b *)
+
+lemma N1_leadsto_b: "|- []($PsiInv & [(N1 | N2) & ~beta1]_(x,y,sem,pc1,pc2))              
+         & SF(N1)_(x,y,sem,pc1,pc2) & [] SF(N2)_(x,y,sem,pc1,pc2)   
+         --> (pc1 = #b | pc1 = #g | pc1 = #a ~> pc1 = #b)"
+  apply (auto intro!: LatticeDisjunctionIntro [temp_use])
+    apply (rule LatticeReflexivity [temp_use])
+   apply (rule LatticeTransitivity [temp_use])
+    apply (auto intro!: a1_leadsto_b1 [temp_use] g1_leadsto_a1 [temp_use]
+      simp: split_box_conj)
+  done
+
+lemma N1_live: "|- []($PsiInv & [(N1 | N2) & ~beta1]_(x,y,sem,pc1,pc2))              
+         & SF(N1)_(x,y,sem,pc1,pc2) & [] SF(N2)_(x,y,sem,pc1,pc2)   
+         --> <>(pc1 = #b)"
+  apply (auto simp: Init_defs intro!: N1_leadsto_b [temp_use, THEN [2] leadsto_init [temp_use]])
+  apply (case_tac "pc1 (st1 sigma)")
+    apply auto
+  done
+
+lemma N1_enabled_at_b: "|- pc1 = #b --> Enabled (<N1>_(x,y,sem,pc1,pc2))"
+  apply clarsimp
+  apply (rule_tac F = beta1 in enabled_mono)
+   apply (tactic {* enabled_tac (thm "Inc_base") 1 *})
+   apply (force simp: beta1_def)
+  apply (force simp: angle_def beta1_def N1_def)
+  done
+
+(* Now assemble the bits and pieces to prove that Psi is fair. *)
+
+lemma Fair_M1_lemma: "|- []($PsiInv & [(N1 | N2)]_(x,y,sem,pc1,pc2))    
+         & SF(N1)_(x,y,sem,pc1,pc2) & []SF(N2)_(x,y,sem,pc1,pc2)   
+         --> SF(M1)_(x,y)"
+  apply (rule_tac B = beta1 and P = "PRED pc1 = #b" in SF2)
+   (* action premises *)
+     apply (force simp: angle_def M1_def beta1_def)
+  apply (force simp: angle_def Psi_defs)
+  apply (force elim!: N1_enabled_at_b [temp_use])
+    (* temporal premise: use previous lemmas and simple TL *)
+  apply (force intro!: DmdStable [temp_use] N1_live [temp_use] Stuck_at_b [temp_use]
+    elim: STL4E [temp_use] simp: square_def)
+  done
+
+lemma Fair_M1: "|- Psi --> WF(M1)_(x,y)"
+  by (auto intro!: SFImplWF [temp_use] Fair_M1_lemma [temp_use] PsiInv [temp_use]
+    simp: Psi_def split_box_conj [temp_use] more_temp_simps)
 
 end
