src/HOL/TLA/Init.thy
@@ -4,9 +4,6 @@
     Author:      Stephan Merz
     Copyright:   1998 University of Munich
 
-    Theory Name: Init
-    Logic Image: HOL
-
 Introduces type of temporal formulas. Defines interface between
 temporal formulas and its "subformulas" (state predicates and actions).
 *)
@@ -43,6 +40,40 @@ defs
   fw_stp_def:  "first_world == st1"
   fw_act_def:  "first_world == %sigma. (st1 sigma, st2 sigma)"
 
-ML {* use_legacy_bindings (the_context ()) *}
+lemma const_simps [int_rewrite, simp]:
+  "|- (Init #True) = #True"
+  "|- (Init #False) = #False"
+  by (auto simp: Init_def)
+
+lemma Init_simps [int_rewrite]:
+  "!!F. |- (Init ~F) = (~ Init F)"
+  "|- (Init (P --> Q)) = (Init P --> Init Q)"
+  "|- (Init (P & Q)) = (Init P & Init Q)"
+  "|- (Init (P | Q)) = (Init P | Init Q)"
+  "|- (Init (P = Q)) = ((Init P) = (Init Q))"
+  "|- (Init (!x. F x)) = (!x. (Init F x))"
+  "|- (Init (? x. F x)) = (? x. (Init F x))"
+  "|- (Init (?! x. F x)) = (?! x. (Init F x))"
+  by (auto simp: Init_def)
+
+lemma Init_stp_act: "|- (Init $P) = (Init P)"
+  by (auto simp add: Init_def fw_act_def fw_stp_def)
+
+lemmas Init_simps = Init_stp_act [int_rewrite] Init_simps
+lemmas Init_stp_act_rev = Init_stp_act [int_rewrite, symmetric]
+
+lemma Init_temp: "|- (Init F) = F"
+  by (auto simp add: Init_def fw_temp_def)
+
+lemmas Init_simps = Init_temp [int_rewrite] Init_simps
+
+(* Trivial instances of the definitions that avoid introducing lambda expressions. *)
+lemma Init_stp: "(sigma |= Init P) = P (st1 sigma)"
+  by (simp add: Init_def fw_stp_def)
+
+lemma Init_act: "(sigma |= Init A) = A (st1 sigma, st2 sigma)"
+  by (simp add: Init_def fw_act_def)
+
+lemmas Init_defs = Init_stp Init_act Init_temp [int_use]
 
 end
