src/HOL/TLA/Memory/MemClerk.thy
@@ -3,12 +3,9 @@
     ID:          $Id$
     Author:      Stephan Merz
     Copyright:   1997 University of Munich
-
-    Theory Name: MemClerk
-    Logic Image: TLA
-
-    RPC-Memory example: specification of the memory clerk.
 *)
+
+header {* RPC-Memory example: specification of the memory clerk *}
 
 theory MemClerk
 imports Memory RPC MemClerkParameters
@@ -67,6 +64,49 @@ constdefs
   MClkISpec     :: "mClkSndChType => mClkRcvChType => mClkStType => temporal"
       "MClkISpec send rcv cst == TEMP (ALL p. MClkIPSpec send rcv cst p)"
 
-ML {* use_legacy_bindings (the_context ()) *}
+lemmas MC_action_defs =
+  MClkInit_def MClkFwd_def MClkRetry_def MClkReply_def MClkNext_def
+
+lemmas MC_temp_defs = MClkIPSpec_def MClkISpec_def
+
+(* The Clerk engages in an action for process p only if there is an outstanding,
+   unanswered call for that process.
+*)
+lemma MClkidle: "|- ~$Calling send p & $(cst!p) = #clkA --> ~MClkNext send rcv cst p"
+  by (auto simp: Return_def MC_action_defs)
+
+lemma MClkbusy: "|- $Calling rcv p --> ~MClkNext send rcv cst p"
+  by (auto simp: Call_def MC_action_defs)
+
+
+(* Enabledness of actions *)
+
+lemma MClkFwd_enabled: "!!p. basevars (rtrner send!p, caller rcv!p, cst!p) ==>  
+      |- Calling send p & ~Calling rcv p & cst!p = #clkA   
+         --> Enabled (MClkFwd send rcv cst p)"
+  by (tactic {* action_simp_tac (simpset () addsimps [thm "MClkFwd_def",
+    thm "Call_def", thm "caller_def", thm "rtrner_def"]) [exI]
+    [thm "base_enabled", Pair_inject] 1 *})
+
+lemma MClkFwd_ch_enabled: "|- Enabled (MClkFwd send rcv cst p)  -->   
+         Enabled (<MClkFwd send rcv cst p>_(cst!p, rtrner send!p, caller rcv!p))"
+  by (auto elim!: enabled_mono simp: angle_def MClkFwd_def)
+
+lemma MClkReply_change: "|- MClkReply send rcv cst p -->  
+         <MClkReply send rcv cst p>_(cst!p, rtrner send!p, caller rcv!p)"
+  by (auto simp: angle_def MClkReply_def elim: Return_changed [temp_use])
+
+lemma MClkReply_enabled: "!!p. basevars (rtrner send!p, caller rcv!p, cst!p) ==>  
+      |- Calling send p & ~Calling rcv p & cst!p = #clkB   
+         --> Enabled (<MClkReply send rcv cst p>_(cst!p, rtrner send!p, caller rcv!p))"
+  apply (tactic {* action_simp_tac (simpset ())
+    [thm "MClkReply_change" RSN (2, thm "enabled_mono") ] [] 1 *})
+  apply (tactic {* action_simp_tac (simpset () addsimps
+    [thm "MClkReply_def", thm "Return_def", thm "caller_def", thm "rtrner_def"])
+    [exI] [thm "base_enabled", Pair_inject] 1 *})
+  done
+
+lemma MClkReplyNotRetry: "|- MClkReply send rcv cst p --> ~MClkRetry send rcv cst p"
+  by (auto simp: MClkReply_def MClkRetry_def)
 
 end
